Update to HHL (from Shuling).

lunarlander/HHL_SL.thy
@@ -5,46 +5,42 @@ theory HHL_SL
 begin
 
 type_synonym now_dash = real
-type_synonym dform = "history \<Rightarrow> now \<Rightarrow> now_dash \<Rightarrow> bool"
+type_synonym 'a dform = "'a history \<Rightarrow> now \<Rightarrow> now_dash \<Rightarrow> bool"
 
-definition semd :: "history \<Rightarrow> now \<Rightarrow> now_dash \<Rightarrow> dform \<Rightarrow> bool" ("_, [_, _] |= _" 50) where
+(*
+definition semd :: "'a history \<Rightarrow> now \<Rightarrow> now_dash \<Rightarrow> 'a dform \<Rightarrow> bool" ("_, [_, _] |= _" 50) where
   "h, [n, m] |= H \<equiv> H h n m"
+*)
 
-text \<open>One axiom stating that the dform formula is only decided by the interval between now and now_dash\<close>
-axiomatization where
-  DC : "now \<le> now' \<Longrightarrow> (\<forall>t. t > now \<and> t < now' \<longrightarrow> h t = h' t) \<Longrightarrow> (df :: dform) h now now' = df h' now now'"
-
+text \<open>The dform formula is only decided by the interval between now and now_dash\<close>
+definition well_DC :: "'a dform \<Rightarrow> bool" where
+"well_DC df == (\<forall> now now' h h'. (now \<le> now' \<and> (\<forall>t. t > now \<and> t < now' \<longrightarrow> h t = h' t)) \<longrightarrow> df h now now' = df h' now now')" 
+ 
 subsection \<open>Duration Calculus operators and lemmas proved\<close>
-
-text \<open>Special assertions \<and> lemmas proved\<close>
-
 text \<open>almost P, P holds everywhere except for the rightmost point, not almost everywhere, over the interval.
 The reason is that, for continuous evolution, it escapes whenever a violation is met.
 A special case is that, if using almost everywhere, the differential cut rule will not hold anymore.\<close>
-definition almost :: "fform \<Rightarrow> dform" where
-(*"almost P \<equiv> % h n nd. (nd-n>0) & (\<not>(\<exists> a b.(n\<le>a & a<b & b\<le>nd) & (\<forall> t. t>a & t<b \<longrightarrow> \<not>P(h(t)))))"*)
-(*An alternative definition of almost*)
-(*"almost P \<equiv> \<lambda>h n nd. (nd-n>0) \<and> (\<forall>a\<ge>n. \<forall>b\<le>nd. a < b \<longrightarrow> (\<exists>t. t>a \<and> t<b \<and> P(h(t))))"*)
-"almost P \<equiv> \<lambda>h n nd. (nd-n>0) \<and> (\<forall>t. t\<ge>n \<and> t < nd \<longrightarrow> P (h (t)))"
+definition almost :: "'a fform \<Rightarrow> 'a dform"  where 
+"almost P \<equiv> \<lambda>h n nd. (nd-n > 0) \<and> (\<forall>t. t \<ge> n \<and> t < nd \<longrightarrow> P (h (t)))"
 
-definition chop :: "dform \<Rightarrow> dform \<Rightarrow> dform"  ("_[^]_" 80) where
-  "chop H M \<equiv> \<lambda>h n nd. \<exists>nm. nm \<ge> n \<and> nm \<le> nd \<and> H h n nm \<and> M h nm nd"
+definition chop :: "'a dform \<Rightarrow> 'a dform \<Rightarrow> 'a dform"  (infixr "[^]" 40) where
+  "H [^] M \<equiv> \<lambda>h n nd. \<exists>nm. nm \<ge> n \<and> nm \<le> nd \<and> H h n nm \<and> M h nm nd"
 
 text \<open>The length of the interval l is equal to, greater than, less than T.\<close>
-definition elE :: "real \<Rightarrow> dform" where
+definition elE :: "real \<Rightarrow> 'a dform" where
   "elE T \<equiv> \<lambda>h n nd. (nd-n) = T"
-definition elG :: "real \<Rightarrow> dform" where
+definition elG :: "real \<Rightarrow> 'a dform" where
   "elG T \<equiv> \<lambda>h n nd. (nd-n) > T"
-definition elL :: "real \<Rightarrow> dform" where
+definition elL :: "real \<Rightarrow> 'a dform" where
   "elL T \<equiv> \<lambda>h n nd. (nd-n) < T"
 
-definition dAnd :: "dform \<Rightarrow> dform \<Rightarrow> dform"  (infixl "[[&]]" 79) where
+definition dAnd :: "'a dform \<Rightarrow> 'a dform \<Rightarrow> 'a dform"  (infixr "[[&]]" 35) where
   "P [[&]] Q \<equiv> \<lambda>h n m. P h n m \<and> Q h n m"
-definition dOr :: "dform \<Rightarrow> dform \<Rightarrow> dform"  (infixl "[[|]]" 79) where
+definition dOr :: "'a dform \<Rightarrow> 'a dform \<Rightarrow> 'a dform"  (infixr "[[|]]" 30) where
   "P [[|]] Q \<equiv> \<lambda>h n m. P h n m \<or> Q h n m"
-definition dNot :: "dform \<Rightarrow> dform"  ("[[\<not>]]_" 79) where
+definition dNot :: "'a dform \<Rightarrow> 'a dform"  ("[[\<not>]]_" 40) where
   "[[\<not>]]P \<equiv> \<lambda>h n m. \<not> P h n m"
-definition dImp :: "dform \<Rightarrow> dform \<Rightarrow> dform"  (infixl "[[\<longrightarrow>]]" 79) where
+definition dImp :: "'a dform \<Rightarrow> 'a dform \<Rightarrow> 'a dform"  (infixr "[[\<longrightarrow>]]" 25) where
   "P [[\<longrightarrow>]] Q \<equiv> \<lambda>h n m. P h n m \<longrightarrow> Q h n m"
 
 declare almost_def [simp]
@@ -66,8 +62,9 @@ lemma chopfb:
   apply (rule conjI, auto)
   by (metis (poly_guards_query) less_eq_real_def less_trans not_less)
 
+text \<open>chop (almost P \/ l = 0) (almost P \/ l = 0) ==> almost P \/ l = 0 \<close>
 lemma chopfor:
-  "chop (elE 0 [[|]]almost P) (elE 0 [[|]]almost P) h n nd \<Longrightarrow> (elE 0 [[|]]almost P) h n nd"
+  "chop (elE 0 [[|]] almost P) (elE 0 [[|]] almost P) h n nd \<Longrightarrow> (elE 0 [[|]] almost P) h n nd"
   unfolding dOr_def
   apply (rule disjCI, auto)
   by (metis less_eq_real_def less_trans not_less)
@@ -84,446 +81,739 @@ lemma chop0L: "chop (almost P) (elE 0) h n nd \<Longrightarrow> almost P h n nd"
 lemma chop0R: "almost P h n nd \<Longrightarrow> chop (almost P) (elE 0) h n nd"
   by auto
 
+lemma chop_well_DC: "well_DC Ha \<Longrightarrow> well_DC Hb \<Longrightarrow> well_DC (Ha [^] Hb)"
+  unfolding chop_def well_DC_def
+  apply auto
+  apply smt
+  apply smt
+  done 
+ 
 text \<open>Monotonicity: s \<Rightarrow> t \<Longrightarrow> almost s \<Rightarrow> almost t\<close>
 lemma almostmono:
   "\<forall>s. P s \<longrightarrow> Q s \<Longrightarrow> \<forall>h n nd. almost P h n nd \<longrightarrow> almost Q h n nd"
   apply auto
-  done 
-
+  by (metis old.prod.exhaust)
+ 
 lemma almostint:
   "now < nowf \<Longrightarrow> \<forall>t. (t\<ge>now \<and> t<nowf) \<longrightarrow> P (f t) \<Longrightarrow> almost P f now nowf"
-  apply auto
-  done  
+  by auto
+
+
 
 subsection \<open>Inference rules for Hybrid CSP: Hybrid Hoare Logic rules\<close>
 
 text \<open>Specification\<close>
-definition Valid :: "fform \<Rightarrow> proc \<Rightarrow> fform \<Rightarrow> dform \<Rightarrow> bool" ("{_}_{_; _}" 80) where
-  "Valid p c q H \<equiv> \<forall>now h now' h'. semB c now h now' h' \<longrightarrow> p (h now) \<longrightarrow> (q (h' now') \<and> H h' now now')"
+definition Valid :: "'a :: finite fform \<Rightarrow> 'a proc \<Rightarrow> 'a fform \<Rightarrow> 'a dform \<Rightarrow> bool" ("\<Turnstile> {_}_{_; _}" 80) where
+  "\<Turnstile> {p} c {q; H} \<longleftrightarrow> (\<forall>now h now' h'. semB c now h now' h' \<longrightarrow> p (h now) \<longrightarrow> (q (h' now') \<and> H h' now now'))"
 
-definition ValidP :: "fform \<Rightarrow> fform \<Rightarrow> procP \<Rightarrow> fform \<Rightarrow> fform \<Rightarrow> dform \<Rightarrow> dform \<Rightarrow> bool"
-  ("{_, _}_{_, _; _, _}" 80) where
-  "ValidP pa pb c qa qb Ha Hb == (\<forall> nowp nowq fp fq nowp' nowq' fp' fq'.
+definition ValidP :: "'a :: finite fform \<Rightarrow> 'a fform \<Rightarrow> 'a procP \<Rightarrow> 'a fform \<Rightarrow> 'a fform \<Rightarrow> 'a dform \<Rightarrow> 'a dform \<Rightarrow> bool"
+  ("\<Turnstile> {_, _}_{_, _; _, _}" 80) where
+  "\<Turnstile> {pa, pb} c {qa, qb; Ha, Hb} \<longleftrightarrow> (\<forall>nowp nowq fp fq nowp' nowq' fp' fq'.
     semBP c nowp fp nowq fq nowp' fp' nowq' fq'  \<longrightarrow> 
-    pa (fp(nowp)) \<longrightarrow>pb (fq(nowq)) \<longrightarrow> 
-    (qa (fp'(nowp'))\<and> qb (fq'(nowq'))\<and> (Ha fp' nowp nowp') \<and> (Hb fq' nowq nowq')))"
+    pa (fp(nowp)) \<longrightarrow> pb (fq(nowq)) \<longrightarrow> 
+    qa (fp'(nowp')) \<and> qb (fq'(nowq')) \<and> (Ha fp' nowp nowp') \<and> (Hb fq' nowq nowq'))"
 
-subsection{*Inference rules proved sound*} 
-
-
-(*Skip rule*)
-lemma SkipRule : "\<forall> s h now now'. (p s \<longrightarrow> q s) \<and> ((elE 0) h now now'\<longrightarrow> H h now now')
-         \<Longrightarrow> {p} Skip {q; H}"
-by (auto simp add:Valid_def)
  
-(*Assignment rule*)
-lemma AssignRRule  :" (\<forall> s. p s \<longrightarrow> (q (% y. if (y = x) then (evalE f s) else s y)))
-                   \<and> (\<forall> h now now'. ((elE 0) h now now'\<longrightarrow> H h now now')) ==>
-       {p} ((RVar x) := f) {q; H}"
-apply (simp add:Valid_def, auto)
-done
-
-(*Sequential rule*)
-(*The proof is complicated because of the existence of chop operator.*)
-lemma SequentialRule_aux : " {p} P {m; H} \<Longrightarrow> {m} Q {q; G} ==>
-             {p} P;  Q {q; H [^] G}" 
-apply  (simp add:Valid_def, auto)
-apply (subgoal_tac "now \<le> now'a \<and> now'a \<le> now'\<and> H h' now now'a = H f' now now'a")
-apply metis
-apply (rule conjI)
-apply (cut_tac P = "P" and now = now and  now'=now'a and f = "h" and f' = "f'" in sem1, simp)
-apply metis
-apply (rule conjI)
-apply (cut_tac P = "Q" and now = now'a and  now'=now' and f = "f'" and f' = "h'" in sem1, simp)
-apply metis
-apply (cut_tac P = "P" and now = now and  now'=now'a and f = "h" and f' = "f'" in sem1, simp)
-apply (cut_tac df = H and now = now and now' = now'a and h = h' and h' = f' in DC, auto)
-apply (cut_tac P = Q in  sem2, auto)
-done
-
-lemma SequentialRule : " {p} P {m; H} \<Longrightarrow> {m} Q {q; G} ==> (\<forall> h m n. (H [^] G) h m n \<longrightarrow> M h m n) \<Longrightarrow>
-             {p} P;  Q {q; M}" 
-apply (cut_tac P = P and  Q = Q  and  p = p and  q =q and m = m and H = H  and  G = G in  SequentialRule_aux, auto)
-apply (simp add:Valid_def)
-done
+text \<open>Partial correctness rules\<close>
+inductive HHL_partial :: "'a :: finite fform \<Rightarrow> 'a proc \<Rightarrow> 'a fform \<Rightarrow> 'a dform \<Rightarrow> bool" ("\<turnstile> {_}_{_; _}" 80) where
+  skipR: "\<forall> s h now now'. (p s \<longrightarrow> q s) \<and> ((elE 0) h now now'\<longrightarrow> H h now now') \<Longrightarrow> well_DC H \<Longrightarrow>
+         \<turnstile>{p} Skip {q; H}"
+| assignR:"(\<forall> s. p s \<longrightarrow> (q (update_fst s x (evalE e s))))
+               \<and> (\<forall> h now now'. ((elE 0) h now now'\<longrightarrow> H h now now')) \<Longrightarrow> well_DC H \<Longrightarrow>
+         \<turnstile> {p} (x := e) {q; H}"
+| seqR: "\<turnstile> {p} P {m; H} \<Longrightarrow> \<turnstile> {m} Q {q; G} ==> (\<forall> h m n. (H [^] G) h m n \<longrightarrow> M h m n) \<Longrightarrow> well_DC M \<Longrightarrow>
+         \<turnstile> {p} P;  Q {q; M}"  
+| condTR: " ((\<forall> s. p s \<longrightarrow> ( b s)) \<and> \<turnstile> {p} P {q; H}) \<Longrightarrow> \<turnstile> {p} IF b P {q; H}"
+| condFR: "((\<forall> s. p s \<longrightarrow> (q s \<and> (\<not>   b s))) \<and> (\<forall> h now now'. ((elE 0) h now now'\<longrightarrow> H h now now')))
+            \<Longrightarrow> well_DC H ==> \<turnstile> {p} IF b P {q; H}"
+| IChoiceR: "\<turnstile> {p} P {m; H} \<Longrightarrow> \<turnstile> {p} Q {q; G} ==> \<turnstile> {p} P \<sqinter> Q {m [|] q; H [[|]] G}"
 
 
-(*Conditional rule*)
-lemma ConditionTRule : " ((\<forall> s. p s \<longrightarrow> ( b s)) \<and> {p} P {q; H})
-             ==> {p} IF b P {q; H}"
-apply (simp add:Valid_def, auto)
-done
-
-lemma ConditionFRule : " ((\<forall> s. p s \<longrightarrow> (q s \<and> (\<not>   b s))) \<and> (\<forall> h now now'. ((elE 0) h now now'\<longrightarrow> H h now now')))
-                          ==> {p} IF b P {q; H}"
-apply (simp add:Valid_def, auto)
-done
-
-lemma ConditionGRule : " {p [&] b} P {q; H} \<and> {p [&] ([\<not>]b)} Q {q; H}
-             ==> {p} IFELSE b P Q{q; H}"
-apply (simp add:Valid_def fAnd_def fNot_def, auto)
-done
-
-declare almost_def [simp del]
-declare chop_def [simp del]
-(*Assume v'=E is the differential equation for the continuous evolution.*)
-(*This proof takes most effort for solving the invariant-related constraints, which will be passed to an 
-external oracle for invariant generation in fact. So don't worry.*)
-lemma ContinuousRule : 
-"\<forall> s u. ( ( \<forall> y. y \<noteq> v \<longrightarrow> s y = u y) \<longrightarrow> (p s) \<longrightarrow> (p u)) \<and>
- ( \<forall> s.  Init s \<longrightarrow>  Inv s)
- \<and> (\<forall> s.  (p [&] (Inv) [&] ([\<not>]b)) s \<longrightarrow> q s)
- \<and> (\<forall> s. (exeFlow (<[v]:E&&Inv&b>) (Inv)) s \<longrightarrow> Inv s)
- \<and>  (\<forall> h now now'. ((elE 0) h now now' \<or> (almost (Inv [&] p  [&] b)) h now now') \<longrightarrow>
-                  H h now now')
- ==> {Init [&] (p::fform)} <[v]:E&&Inv&(b)> {q; H}"
-apply (simp add:Valid_def) apply clarify
-apply (subgoal_tac "\<forall> t. t\<ge>now & t\<le>now' \<longrightarrow> exeFlow (<[v]:E&&Inv&b>) (Inv) (h'(t))")
-prefer 2
-apply (simp add:exeFlow_def)
-apply (metis fAnd_def)
-apply auto
-apply (metis fAnd_def)
-apply (subgoal_tac "(p [&] Inv) (\<lambda> y. if y = v then Solution (Flow [v] E) (h now) (now + d - now) else h now y)")
-apply (simp add:fAnd_def)+
-apply (rule conjI, auto)
-apply (subgoal_tac "\<forall> y.  y \<noteq> v \<longrightarrow> (h(now)) y = ((\<lambda> y. if y = v 
-   then Solution (Flow [v] E) (h now) (now + d - now) else h now y)) y")
-apply smt     
-apply auto 
-apply (subgoal_tac "exeFlow (<[v]:E&&Inv&b>) (Inv)
-                    (\<lambda> y. if y =  v 
-        then Solution (Flow [v] E) (h now) (now+d - now) else h now y)")
-apply (metis (no_types, lifting))
-apply (drule_tac x = "now +d" in spec, auto)
-apply (subgoal_tac "almost (Inv [&] p [&] b) 
-(\<lambda>t. if t \<le> now + d \<and> now < t then \<lambda> y. if y = v 
-then Solution (Flow [v] E) (h now) (t - now) else h now y else h t) now (now+d)", auto)
-apply (rule almostint, auto)
-apply (simp add:fAnd_def)
-apply (rule conjI)
-apply (subgoal_tac "exeFlow (<[v]:E&&Inv&b>) (Inv)
-                    (\<lambda> y. if y = v 
-        then Solution (Flow [v] E) (h now) (t - now) else h now y)")
-apply (metis (no_types, lifting)) 
-apply (drule_tac x = "t" in spec, auto)
-apply (subgoal_tac "\<forall> y. y \<noteq> v \<longrightarrow> (h(now)) y = ((\<lambda> y. if y = v 
-   then Solution (Flow [v] E) (h now) (t - now) else h now y)) y")
-apply smt
-apply auto
-by (smt fAnd_def) 
-
-(*We simple extend the above rule to the general case where the continuous are a list of variables not just one.
-The proof can be given in the same way.*)
-primrec notcontain :: "string \<Rightarrow> string list \<Rightarrow> bool" 
-where
-"notcontain a ([]) = True" |
-"notcontain a (e # Elist) = (if a = e then False else (notcontain a Elist))"
-
-axiomatization where ContinuousRuleGT:
-" (\<forall> s. (p) s --> b s)
-\<and> ( \<forall> s.  p s \<longrightarrow>  Inv s)
- \<and> (\<forall> s.  ((Inv) [&] (close (b)) [&] (close([\<not>]b))) s \<longrightarrow> q s)
- \<and> (\<forall> s. (exeFlow (<V:E&&Inv&b>) (Inv)) s \<longrightarrow> Inv s)
- \<and>  (\<forall> h now now'. ((elE 0) h now now' \<or> (almost (Inv [&]  close(b))) h now now') \<longrightarrow>
-                  H h now now')
- ==> {p} <V:E&&Inv&(b)> {q; H}"
-
-axiomatization where ContinuousRuleGF:
-" \<forall> s. p s \<longrightarrow> (([\<not>] b) [&]q) s
- ==> {p} <V:E&&Inv&(b)> {q; elE 0}"
 
 
-text \<open>Shallow definition: a variable does not affect the formula \<close>
-definition not_in_fform:: "string \<Rightarrow> fform \<Rightarrow> bool"  where
-  "not_in_fform w P = (\<forall> s u. ((\<forall> y. y \<noteq> w \<longrightarrow> s y = u y)) \<longrightarrow> (P s \<longleftrightarrow> P u))"
+| repetR: "\<forall>h n m. (H[^]H) h n m \<longrightarrow> H h n m \<Longrightarrow> \<turnstile> {I} P {I; H}  \<Longrightarrow> 
+           \<turnstile> {I} P*&&I {I; (H [[|]] (elE 0))} "
 
-definition not_in_dform:: "string \<Rightarrow> dform \<Rightarrow> bool"  where
-  "not_in_dform w Q = (\<forall>h l n nd. ((\<forall> y. y \<noteq> w \<longrightarrow> (\<forall> t. t \<ge> n \<and> t \<le> nd \<longrightarrow> h(t) y = l(t) y)))
-  \<longrightarrow> ((Q h n nd \<longrightarrow> Q l n nd) \<and> (Q l n nd \<longrightarrow> Q h n nd)))"
+| consequenceR: "\<turnstile> {px} P {qx; Hx} \<Longrightarrow> (\<forall> s. p s \<longrightarrow> px s) \<Longrightarrow> (\<forall> s. qx s \<longrightarrow> q s) \<Longrightarrow>
+                 (\<forall> h n m. Hx h n m \<longrightarrow> H h n m) \<Longrightarrow> well_DC H \<Longrightarrow> \<turnstile> {p} P {q; H}"
 
-lemma not_in_fform_update:
-  "not_in_fform w P \<Longrightarrow> P (\<lambda>y. if y \<noteq> w then s y else c) \<longleftrightarrow> P s"
-  by (simp add: not_in_fform_def)
+| continTR: "\<forall> s. (Inv [&][\<not>]b) s \<longrightarrow> q s \<Longrightarrow>
+             \<forall> s. p s  \<longrightarrow> ODE_inv_in_dom ode s b Inv \<Longrightarrow>
+             \<forall> h now now'. (almost (Inv [&]  b) [[|]] elE 0) h now now' \<longrightarrow>
+               H h now now' \<Longrightarrow> well_DC H  \<Longrightarrow> 
+             \<turnstile> {p} <ode && Inv&b> {q; H}"
 
-lemma not_in_dform_update:
-  "not_in_dform w Q \<Longrightarrow> Q (\<lambda>t. if t \<le> nd \<and> n \<le> t then \<lambda>y. if y \<noteq> w then h t y else l t y else h t) n nd \<longleftrightarrow> Q h n nd"
-  apply (simp add:not_in_dform_def)
-  by smt
+|diffCut: "\<turnstile> {p} <ode && Inv&b> {I; almost I [[|]] elE 0} \<Longrightarrow> 
+               \<turnstile> {p} <ode && Inv&(b[&]I)> {q; H} \<Longrightarrow>
+               \<turnstile> {p} <ode && Inv&b> {q; H}"
 
-text \<open>Ghost rule for continuous evolution\<close>
-lemma GhostRule : 
-  assumes "(w \<notin> set VL)"
-    and "not_in_fform w p"
-    and "not_in_fform w q"
-    and "not_in_dform w H"    
-    and "{pre} <(VL@[w]):(EL@[F])&&Inv&(b)> {post; HF}"
-    and " \<forall> s. \<exists> a. (let sa = (\<lambda> y. (if y \<noteq> w then s y else a)) in p s \<longleftrightarrow>  pre sa)"
-    and "\<forall> s. \<exists> a. (let sa = (\<lambda> y. (if y \<noteq> w then s y else a)) in  q s \<longleftrightarrow> post sa)"
-    and "\<forall>h n nd. \<exists> xa. (let ha = (\<lambda>t. if t \<le> nd \<and> n \<le> t then (\<lambda> y. (if y \<noteq> w then h t y else xa t y)) else h t)
-           in  H h n nd \<longleftrightarrow> HF ha n nd)"
-  shows "{p} <VL:EL&&Inv&(b)> {q; H}"
-  sorry
 (*
+Different from Platzer's: This is not valid when b always be true. 
+|diffCut2: "\<turnstile> {p} <ode && Inv&b> {I; almost I [[|]] elE 0} \<Longrightarrow> 
+                \<turnstile> {p} <ode && Inv&b> {q; H} \<Longrightarrow>
+                \<turnstile> {p} <ode && Inv&(b[&]I)> {q; H}"
+*)
+
+(*This is different from Platzer's: not b holds at the termination.*)
+|diffWeak: "\<forall> h now now'. (almost b [[|]] elE 0) h now now' \<longrightarrow>
+            H h now now' \<Longrightarrow> well_DC H \<Longrightarrow> \<turnstile> {p} <ode && Inv&b> {[\<not>]b; H}"
+
+|diffE: "\<turnstile> {p} <odeone x e && Inv & b>; DAss x e {b; H} \<Longrightarrow> DE_free e \<Longrightarrow>
+         \<turnstile> {p} <odeone x e && Inv & b> {b; H}"
+
+|diffE2: "\<turnstile> {p} <odeone x e && Inv & b> {b; H} \<Longrightarrow> DE_free e \<Longrightarrow>
+          \<turnstile> {p} <odeone x e && Inv & b>; DAss x e {b; H}"
+(*
+|diffSol: "\<forall> s. \<forall> t\<ge>0 .\<forall> u. u\<ge>0 \<and> u\<le>t \<longrightarrow> b(s) \<Longrightarrow> well
+           \<turnstile> {p} <odeone x e && Inv & b> {b; H}"
+*)
+
+|diffInvGE: "\<forall> s. b s \<longrightarrow> q s \<Longrightarrow> 
+           \<turnstile> {p} <odeone x e && Inv & b> {(Diff f1) [\<ge>] (Diff f2); (almost ((Diff f1) [\<ge>] (Diff f2)) [[|]] elE 0)} \<Longrightarrow>
+           \<forall> h now now'. (almost (f1 [\<ge>] f2) [[|]] elE 0) h now now' \<longrightarrow>
+            H h now now' \<Longrightarrow> well_DC H \<Longrightarrow>
+           \<turnstile> {p} <odeone x e && Inv & b> {f1 [\<ge>] f2; H}"
+
+|diffInvG: "\<forall> s. b s \<longrightarrow> q s \<Longrightarrow> 
+           \<turnstile> {p} <odeone x e && Inv & b> {(Diff f1) [>] (Diff f2); (almost ((Diff f1) [>] (Diff f2)) [[|]] elE 0)} \<Longrightarrow>
+           \<forall> h now now'. (almost (f1 [>] f2) [[|]] elE 0) h now now' \<longrightarrow>
+            H h now now' \<Longrightarrow> well_DC H \<Longrightarrow>
+           \<turnstile> {p} <odeone x e && Inv & b> {f1 [>] f2; H}"
+
+|diffGhost: "\<forall> s. b s \<longrightarrow> q s \<Longrightarrow> 
+           \<turnstile> {p} <odeone x e && Inv & b> {q; (almost q [[|]] elE 0)} \<Longrightarrow>
+           \<forall> h now now'. (almost q [[|]] elE 0) h now now' \<longrightarrow>
+            H h now now' \<Longrightarrow> well_DC H \<Longrightarrow>
+           \<turnstile> {p} <odeone x e && Inv & b> {q; H}"
+
+|caseR: "\<turnstile> {p [&] pb} P {q; H} \<Longrightarrow> \<turnstile> {(p [&] ([\<not>]pb))} P {q; H} \<Longrightarrow>
+             \<turnstile> {p} P {q; H}"
+
+
+ 
+text \<open>When two independent P and Q are put in parallel, \<close>
+text \<open>and when a communication follows P and Q,\<close>
+text \<open>and when P and Q contain communication, and U V not.\<close>
+inductive HHL_para :: "'a :: finite fform \<Rightarrow> 'a fform \<Rightarrow> 'a procP \<Rightarrow> 
+  'a fform \<Rightarrow> 'a fform \<Rightarrow> 'a dform \<Rightarrow> 'a dform \<Rightarrow> bool" ("\<turnstile> {_, _}_{_, _; _, _}" 70) where
+  parallelR: "chanset P = {} \<and> chanset Q = {} \<Longrightarrow> \<turnstile> {pp} P {qp; Hp} \<Longrightarrow> \<turnstile> {pq} Q {qq; Hq}
+                       \<Longrightarrow> \<turnstile> {pp, pq} P||Q {qp, qq; Hp, Hq}"
+
+| commR: "\<turnstile> {px, py} (P || Q) {qx, qy; Hx, Hy} \<Longrightarrow>  
+         (\<forall> s. qx s \<longrightarrow> (rx (update_fst s x (evalE e s)))) \<Longrightarrow>
+         (\<forall> s. qy s \<longrightarrow> ry s) \<Longrightarrow>
+         (\<forall> h n m. (Hx[^](elE 0 [[|]] almost qx)) h n m \<longrightarrow> Gx h n m) \<Longrightarrow>
+         (\<forall> h n m. (Hy[^](elE 0 [[|]] almost qy)) h n m \<longrightarrow> Gy h n m) \<Longrightarrow>
+          well_DC Gx \<and> well_DC Gy \<Longrightarrow>
+          \<turnstile> {px, py} (P; Cm (ch[?]x))||(Q; (Cm (ch[!]e))) {rx, ry; Gx, Gy}"
+
+| parallel2R: "\<turnstile> {pp, pq} P||Q {qp, qq; Hp, Hq}  \<Longrightarrow> chanset P \<noteq> {} \<and> chanset Q \<noteq> {} \<Longrightarrow> 
+               \<turnstile> {qp} U {qu; Hu} \<Longrightarrow> \<turnstile> {qq} V {qv; Hv} \<Longrightarrow> chanset U = {} \<and> chanset V = {} 
+              \<Longrightarrow> \<turnstile> {pp, pq} P; U||Q; V {qu, qv; Hp [^] Hu, Hq [^] Hv}"
+
+
+lemma hhl_well_DC : "\<turnstile> {p} P {q; H} \<Longrightarrow> well_DC H"
+proof (induction rule: HHL_partial.induct)
+  case (IChoiceR p P m H Q q G)
+  then show ?case
+    unfolding dOr_def well_DC_def
+    by blast
+
+next
+  case (repetR H I P)
+  then show ?case
+    unfolding well_DC_def dOr_def
+    by (metis (mono_tags, lifting) elE_def)
+
+qed auto
+
+
+lemma hhl_well_DC_par : "\<turnstile> {pp, pq} P||Q {qp, qq; Hp, Hq}  \<Longrightarrow> well_DC Hp \<and> well_DC Hq"
+proof (induction rule: HHL_para.induct)
+case (parallelR P Q pp qp Hp pq qq Hq)
+  then show ?case
+    using hhl_well_DC by auto
+next
+  case (commR px py P Q qx qy Hx Hy rx x e ry Gx Gy ch)
+  then show ?case by auto
+next
+  case (parallel2R pp pq P Q qp qq Hp Hq U qu Hu V qv Hv)
+  then have Hpq: "well_DC Hp \<and> well_DC Hq" 
+    and Huv: "well_DC Hu \<and> well_DC Hv" using hhl_well_DC by auto
+  show ?case using Hpq Huv chop_well_DC by auto
+qed
+
+(*Sequential*)
+lemma Sequential_aux : 
+  assumes "well_DC H" and "\<turnstile> {p} P {m; H}" and "\<turnstile> {m} Q {q; G}" and 
+    "\<Turnstile> {p} P {m; H}" and "\<Turnstile> {m} Q {q; G}"
+  shows "\<Turnstile> {p} P;  Q {q; H [^] G}" 
 proof -
-  have "\<forall>now h now' h'.
-       semB (<[v, w]:[E, F]&&Inv&b>) now h now' h' \<longrightarrow>
-       (Init [&] p) (h now) \<longrightarrow> q (h' now') \<and> H h' now now'"
-    using assms(4) unfolding Valid_def by auto
-  have "\<forall>now h now' h'.
-       semB (<[v]:[E]&&Inv&b>) now h now' h' \<longrightarrow> (Init [&] p) (h now) \<longrightarrow> q (h' now') \<and> H h' now now'"
+  have "\<forall>now h now' h'. semB (P; Q) now h now' h' \<longrightarrow> p (h now) \<longrightarrow> 
+    q (h' now') \<and> (\<exists>nm\<ge>now. nm \<le> now' \<and> H h' now nm \<and> G h' nm now')"
   proof -
     {
-      fix now h now' h'
-      assume semE: "semB (<[v]:[E]&&Inv&b>) now h now' h'"
-        and Init: "(Init [&] p) (h now)" 
-      define nowf where "nowf = now'"
-      
-      have semEF: "\<exists> hf. semB (<[v, w]:[E, F]&&Inv&b>) now h nowf hf \<and> 
-        ((\<forall> y i.(y, i) \<noteq> (fst (w), snd (w)) \<longrightarrow> (\<forall> t. t \<ge> now \<and> t \<le> nowf \<longrightarrow> hf(t) (y, i) = h'(t) (y, i))))"
-        sorry 
-      then obtain hf where 
-        EF: "semB (<[v, w]:[E, F]&&Inv&b>) now h nowf hf"
-        and hfh: "((\<forall> y i.(y, i) \<noteq> (fst (w), snd (w)) \<longrightarrow> (\<forall> t. t \<ge> now \<and> t \<le> nowf \<longrightarrow> hf(t) (y, i) = h'(t) (y, i))))"
-        and post: "q (hf nowf) \<and> H hf now nowf"
-        using assms(4) Init unfolding Valid_def by auto
-      have  "((\<forall> y i.(y, i) \<noteq> (fst (w), snd (w)) \<longrightarrow> hf(nowf) (y, i) = h'(nowf) (y, i)))"
-      proof -
-        {
-          fix y i assume yi: "(y, i) \<noteq> (fst (w), snd (w))"
-          have "(\<forall> t. t \<ge> now \<and> t \<le> nowf \<longrightarrow> hf(t) (y, i) = h'(t) (y, i))" using hfh yi by auto
-          then have "hf(nowf) (y, i) = h'(nowf) (y, i)" using EF sem1 by auto
-        }
-        then show ?thesis by auto
-      qed
-      then have qf: "q (h' now')" using post assms(2) not_in_fform_def unfolding nowf_def by auto
-      then have Hf: "q (h' now') \<and> H h' now now'" using assms(3) hfh post unfolding not_in_dform_def nowf_def by blast
+      fix now h now' h' 
+      assume PQ: "semB (P; Q) now h now' h'" and pre: "p (h now)"
+      obtain now'a f' where sP: "semB P now h now'a f'" and sQ: "semB Q now'a f' now' h'" 
+        using PQ by clarsimp
+      have post: "m (f' now'a) \<and> H f' now now'a \<and> q (h' now') \<and> G h' now'a now'" 
+        using sP sQ pre assms unfolding Valid_def by auto 
+      have nowa: "now \<le> now'a" using sP by (simp add: sem1)
+      moreover have hf: "(now'a \<le> now' \<and> (\<forall>t. t < now'a \<or> t > now' \<longrightarrow> f' t = h' t))"
+        using sQ by (simp add: sem1 sem2)
+      ultimately have "now \<le> now' \<and> (\<forall>t. now < t \<and> t < now'a \<longrightarrow> f' t = h' t)" by auto
+      then have "H h' now now'a" using assms(1) post nowa unfolding well_DC_def by auto
+      then have "q (h' now') \<and> (\<exists>nm\<ge>now. nm \<le> now' \<and> H h' now nm \<and> G h' nm now')"
+        using post hf nowa by blast       
     }
     then show ?thesis by auto
   qed
-  then show ?thesis unfolding Valid_def by auto
+  then show ?thesis  unfolding Valid_def chop_def by auto
 qed
-*)
 
-lemma DiffCutRule : 
-  assumes I: "{p} <[v]:E&&Inv&(b)> {I; almost I [[|]] elE 0}"
-    and C: "{p} <[v]:E&&Inv&(b[&]I)> {q; H}"
-  shows "{p} <[v]:E&&Inv&(b)> {q; H}"
-proof (simp add:Valid_def, clarify)  
-  have "\<forall>now h now' h'. semB (<[v]:E&&Inv&b>) now h now' h' \<longrightarrow> p (h now) 
+lemma repetitionN_0:
+  " \<forall>h n m. (H[^]H) h n m \<longrightarrow> H h n m \<Longrightarrow>
+    \<turnstile> {I}P{I; H} \<Longrightarrow>
+   \<forall>now h now' h'. semB P now h now' h' \<longrightarrow> I (h now) \<longrightarrow> I (h' now') \<and> H h' now now' \<Longrightarrow>
+    semB (P* NUM 0) now h now' h' \<Longrightarrow> I (h now) \<Longrightarrow> I (h' now') \<and> (H h' now now' \<or> elE 0 h' now now')"
+  apply (ind_cases "semB (P* NUM 0) now h now' h'")
+  unfolding elE_def
+  by fastforce
+
+lemma repetitionN_Suc: 
+assumes incN: "(\<And>now h now' h'.
+           \<forall>h n m. (H[^]H) h n m \<longrightarrow> H h n m \<Longrightarrow>
+           \<turnstile> {I}P{I; H} \<Longrightarrow>
+           \<forall>now h now' h'. semB P now h now' h' \<longrightarrow> I (h now) \<longrightarrow> I (h' now') \<and> H h' now now' \<Longrightarrow>
+           semB (P* NUM N) now h now' h' \<Longrightarrow> I (h now) \<Longrightarrow> I (h' now') \<and> (H h' now now' \<or> elE 0 h' now now'))"
+  and chopH: "\<forall>h n m. (H[^]H) h n m \<longrightarrow> H h n m"
+  and rP: "\<turnstile> {I} P {I; H}"
+  and semBP: "\<forall>now h now' h'. semB P now h now' h' \<longrightarrow> I (h now) \<longrightarrow> I (h' now') \<and> H h' now now'"
+(*  and semBPP: "semB (P* NUM Suc N) now h now' h'"
+  and pre: "I (h now)"
+shows "I (h' now') \<and> (H h' now now' \<or> elE 0 h' now now')"
+*)
+shows "semB (P* NUM Suc N) now h now' h' \<Longrightarrow> I (h now) \<Longrightarrow> I (h' now') \<and> (H h' now now' \<or> elE 0 h' now now')"
+proof (ind_cases "semB (P* NUM Suc N) now h now' h'")
+  have wellH: "well_DC H" using hhl_well_DC rP by auto
+  have Pf: "\<And>now_d f_d. I (h now) \<Longrightarrow> semB P now h now_d f_d \<Longrightarrow>  I (f_d now_d) \<and> H f_d now now_d"
+    using semBP by auto
+
+   have PNf: "\<And>now_d f_d. semB (P* NUM N) now_d f_d now' h' \<Longrightarrow> I (f_d now_d) \<Longrightarrow> I (h' now') \<and> (H h' now_d now' \<or> elE 0 h' now_d now')"
+     using incN[of _ _ now' h'] chopH rP semBP by metis
+   have PPNf: "\<And>now_d f_d. semB P now h now_d f_d \<Longrightarrow> semB (P* NUM N) now_d f_d now' h' \<Longrightarrow> H f_d now now_d = H h' now now_d"
+     using wellH unfolding well_DC_def 
+     by (simp add: sem1 sem2)
+   have "\<And>now_d f_d. I (h now) \<Longrightarrow> semB P now h now_d f_d \<Longrightarrow> semB (P* NUM N) now_d f_d now' h'\<Longrightarrow> I (h' now') \<and> H h' now now'" 
+     using PNf Pf PPNf chopH unfolding elE_def chop_def 
+     by (metis eq_iff le_iff_diff_le_0 sem1)
+   then show "\<And>now_d f_d. I (h now) \<Longrightarrow> semB P now h now_d f_d \<Longrightarrow> semB (P* NUM (Suc N - Suc 0)) now_d f_d now' h' 
+              \<Longrightarrow> I (h' now') \<and> (H h' now now' \<or> elE 0 h' now now')"
+     by auto
+ qed
+
+lemma repetitionN_sound: 
+  "\<forall>h n m. (H[^]H) h n m \<longrightarrow> H h n m \<Longrightarrow>
+       \<turnstile> {I}P{I; H} \<Longrightarrow>
+       \<forall>now h now' h'. semB P now h now' h' \<longrightarrow> I (h now) \<longrightarrow> I (h' now') \<and> H h' now now' \<Longrightarrow>
+       semB (P* NUM N) now h now' h' \<Longrightarrow> I (h now) \<Longrightarrow> I (h' now') \<and> (H [[|]] elE 0) h' now now'"
+  unfolding dOr_def
+  apply (induction N arbitrary: now h now' h')
+  subgoal
+  using repetitionN_0[of H I P] by metis
+  using repetitionN_Suc[of H I P]
+  by smt 
+      
+lemma diffCut_aux : 
+  assumes I: "\<turnstile> {p}<ode&&Inv&b>{I; almost I [[|]] elE 0}" 
+    and vI: "\<Turnstile> {p}<ode&&Inv&b>{I; almost I [[|]] elE 0}"
+    and C: "\<turnstile> {p}<ode&&Inv&(b [&] I)>{q; H}"
+    and vC: "\<Turnstile> {p}<ode&&Inv&(b [&] I)>{q; H}"
+  shows "\<Turnstile> {p} <ode&&Inv&b> {q; H}"
+proof (simp add:Valid_def) 
+  have "\<forall>now h now' h'. semB (<ode&&Inv&b>) now h now' h' \<longrightarrow> p (h now) 
     \<longrightarrow> I (h' now') \<and> (almost I [[|]] elE 0) h' now now'"
-    using I unfolding Valid_def by auto
-  have semI: "semB (<[v]:E&&Inv&b>) now h now' h' \<Longrightarrow> p (h now) \<Longrightarrow> semB (<[v]:E&&Inv&b [&] I>) now h now' h'"
+    using vI unfolding Valid_def by auto
+  have semI: "semB (<ode&&Inv&b>) now h now' h' \<Longrightarrow> p (h now) \<Longrightarrow> semB (<ode&&Inv&(b [&] I)>) now h now' h'"
     for now h now' h'
-    apply (ind_cases "semB (<[v]:E&&Inv&b>) now h now' h'")
-    subgoal 
-    proof -
-      assume a: "p (h now)" and b: "now' = now" and c: "h' = h" and d: "([\<not>]b) (h now)"
-      show "semB (<[v]:E&&Inv&b [&] I>) now h now' h'"
-      proof -
-        have "([\<not>] (b [&] I)) (h now)" using d unfolding fNot_def fAnd_def by auto
-        then show ?thesis
-          by (simp add: b c continuousBF)
-      qed
-    qed
-    subgoal for d
+    apply (ind_cases "semB (<ode&&Inv&b>) now h now' h'")
+    subgoal for d sol
     proof -
       assume a: "p (h now)" and b: "now' = now + d"  
-        and c: "h' = (\<lambda>t. if t \<le> now + d \<and> now < t then \<lambda> y. if y = v then Solution (Flow [v] E) (h now) (t - now) else h now y else h t)"
-        and d: "0 < d" and e: "\<forall>m. m < now + d \<and> now \<le> m \<longrightarrow>
-          b (if now < m then \<lambda> y. if y = v then Solution (Flow [v] E) (h now) (m - now) else h now y else h m)"
-        and f: "([\<not>]b) (\<lambda> y. if y = v then Solution (Flow [v] E) (h now) (now + d - now) else h now y)"
-      show "semB (<[v]:E&&Inv&b [&] I>) now h now' h'"
+        and c: "h' = (\<lambda>t. if t \<le> now + d \<and> now \<le> t then  execute_ODE ode (h now) (sol (t - now)) else h t)"
+        and d: "0 \<le> d" 
+        and s: "ODE_solution ode d (h now) sol"
+        and e: "(\<forall>t. 0 \<le> t \<and> t < d \<longrightarrow> b (execute_ODE ode (h now) (sol t)))"
+        and f: "\<not> b (execute_ODE ode (h now) (sol d)) "
+      show "semB (<ode&&Inv&(b [&] I)>) now h now' h'"
       proof -
-        have "semB (<[v]:E&&Inv&b>) now h (now + d) h'" 
-          using b c d e f continuousBT[of d now v  E h b Inv] by auto
-        then have "I (h' now') \<and> (almost I [[|]] elE 0) h' now now'" 
-          using a I b unfolding Valid_def by auto
-        then have almostI: "I (h' now') \<and> (almost I) h' now now'" 
-          using b c d unfolding elE_def dOr_def by auto
-        have "([\<not>] (b [&] I))(h' (now + d))"
-          using f d c unfolding fNot_def fAnd_def by auto
-        moreover have "\<forall>m. m < now + d \<and> now \<le> m \<longrightarrow> (b [&] I) (h' (m))"
-          using almostI b e c unfolding almost_def fAnd_def by auto
-        ultimately show ?thesis using b c d continuousBT[of d now v  E h "b[&]I" Inv] unfolding Let_def 
-          by auto
-      qed
+        have "semB (<ode&&Inv&b>) now h (now + d) h'" 
+          using b c d e s f continuous by auto
+        then have almostI: "I (h' now') \<and> (almost I [[|]] elE 0) h' now now'" 
+          using a vI b unfolding Valid_def by auto
+        have "\<not> (b [&] I) (execute_ODE ode (h now) (sol d))"
+          using e d c f unfolding fNot_def fAnd_def by auto
+        moreover have "\<forall>t. 0 \<le> t \<and> t < d \<longrightarrow> (b [&] I) (execute_ODE ode (h now) (sol t))"
+          using almostI  d b e c unfolding almost_def fAnd_def Let_def dOr_def elE_def 
+          by smt
+        ultimately have "(\<forall>t. 0 \<le> t \<and> t < d \<longrightarrow> b (execute_ODE ode (h now) (sol t)) \<and> 
+          I (execute_ODE ode (h now) (sol t))) \<and>
+          \<not> (b (execute_ODE ode (h now) (sol d)) \<and> I (execute_ODE ode (h now) (sol d)))" 
+          unfolding fAnd_def by auto      
+        then show ?thesis        
+          using b s c d continuous[of d ode h now sol "b[&]I" Inv]  unfolding Let_def fAnd_def
+          by auto       
+     qed
     qed
     done
 
-  have "semB (<[v]:E&&Inv&b>) now h now' h' \<Longrightarrow> p (h now) \<Longrightarrow> q (h' now') \<and> H h' now now'"
+  have "semB (<ode&&Inv&b>) now h now' h' \<Longrightarrow> p (h now) \<Longrightarrow> q (h' now') \<and> H h' now now'"
     for now h now' h'
-    using C semI unfolding Valid_def by meson
-  then show "\<And>now h now' h'. semB (<[v]:E&&Inv&b>) now h now' h' \<Longrightarrow> p (h now) \<Longrightarrow> q (h' now') \<and> H h' now now'"
+    using vC semI unfolding Valid_def by meson
+  then show "\<forall>now h now' h'. semB (<ode&&Inv&b>) now h now' h' \<longrightarrow> p (h now) \<longrightarrow> q (h' now') \<and> H h' now now'"
     by auto
 qed 
 
-(*There are three rules for parallel  composition, which covers all the cases.*)
-(*Parallel rule for the case without communication*)
-lemma Parallel1Rule : "chanset P = {} \<and> chanset Q = {} \<Longrightarrow> {pp} P {qp; Hp} \<Longrightarrow> {pq} Q {qq; Hq}
-                       \<Longrightarrow> {pp, pq} P||Q {qp, qq; Hp, Hq}"
-apply (clarsimp simp:Valid_def ValidP_def)
-by (meson semB3)
+lemma has_vderiv_on_zero_partial_constant:
+  fixes f :: "real \<Rightarrow> ('a :: finite) state"
+  assumes solv: "(f has_vderiv_on (\<lambda>xa. \<chi> i. if i = x then M (f xa) else 0)) {0..d}"
+    and xi:  "i \<noteq> x"
+    and tv: "t \<ge> 0  & t \<le> d"
+  shows "f t $ i = f 0 $ i"
+  sorry
 
-(*Parallel rule for the case with communication at the end.*)
-lemma Communication_aux: 
-"  semBP (P; Cm (ch??(RVar x)) || Q; Cm (ch!!e)) nowp fp nowq fq nowp' fp' nowq' fq' \<Longrightarrow>
-    \<forall> nowp nowq fp fq nowp' nowq' fp' fq'.
-          semBP (P || Q) nowp fp nowq fq nowp' fp' nowq' fq' \<longrightarrow>
-          px (fp nowp) \<longrightarrow> py (fq nowq) \<longrightarrow> qx (fp' nowp') \<and> qy (fq' nowq') \<and> Hx fp' nowp nowp' \<and> Hy fq' nowq nowq' \<Longrightarrow>
-       \<forall>s. qx s \<longrightarrow> rx (\<lambda> y. if y = x then evalE e s else s y) \<Longrightarrow>
-       \<forall>s. qy s \<longrightarrow> ry s \<Longrightarrow>
-       \<forall>h n m. (Hx[^](elE 0 [[|]]almost qx)) h n m \<longrightarrow> Gx h n m \<Longrightarrow>
-       \<forall>h n m. (Hy[^](elE 0 [[|]]almost qy)) h n m \<longrightarrow> Gy h n m \<Longrightarrow>      
-       px (fp nowp) \<Longrightarrow> py (fq nowq) \<Longrightarrow> rx (fp' nowp') \<and> ry (fq' nowq') \<and> Gx fp' nowp nowp' \<and> Gy fq' nowq nowq'"
-apply (ind_cases "semBP (P; Cm (ch??(RVar x)) || Q; Cm (ch!!e)) nowp fp nowq fq nowp' fp' nowq' fq'")
+lemma ODE_only_changes_not_zero_deriv: 
+  assumes "ODE_solution (odeone x e) d (aa, bb) sol"
+    and tv: "t \<ge> 0  & t \<le> d"
+  shows "sol t = fst (execute_ODE (odeone x e) (aa, bb) (sol t))"
+proof -
+  have "sol t = fst (concrete_sol (odeone x e) (aa, bb) (sol t))"
+    using assms 
+    unfolding ODE_solution_def concrete_sol_def ODE_pair_state_def 
+    apply auto
+    using vec_eq_iff[of "sol t" "(\<chi> i. (if i = x then sol t else fst (aa, bb)) $ i)"]
+    apply auto
+    subgoal for i
+      using has_vderiv_on_zero_partial_constant[of sol x _ d i t]  by auto
+    done
+  then show ?thesis using execute_ODE_concrete by metis   
+qed
+
+  
+lemma diffE_lemma: 
+  fixes e :: "('a :: finite) exp"
+    and aa bb :: "'a state"
+    and sol :: "real \<Rightarrow> 'a state"
+  assumes DEf: "DE_free e"
+    and solx: "ODE_solution (odeone x e) d (aa, bb) sol"
+    and tv: "t \<ge> 0  & t \<le> d"
+  shows "evalE e (execute_ODE (odeone x e) (aa, bb) (sol t)) =
+            snd (execute_ODE (odeone x e) (aa, bb) (sol t)) $ x"
+proof -
+  have agree: "Vagree (execute_ODE (odeone x e) (aa, bb) (sol t)) (ODE_pair_state (odeone x e) (sol t)) {x}"
+    using execute_ODE_agree[of "odeone x e" "(aa, bb)" "sol t"]
+    by auto
+  then have "snd (execute_ODE (odeone x e) (aa, bb) (sol t)) $ x = 
+             ODE_sem (odeone x e) (sol t) $ x"
+    unfolding Vagree_def ODE_pair_state_def by auto
+  moreover have "ODE_sem (odeone x e) (sol t) $ x = evalE_df e (sol t)"
+    by auto
+  moreover have "evalE e (execute_ODE (odeone x e) (aa, bb) (sol t)) =
+        evalE_df e (fst (execute_ODE (odeone x e) (aa, bb) (sol t)))"
+    using DEf by (simp add: DE_free_evalE)
+  moreover have "fst (execute_ODE (odeone x e) (aa, bb) (sol t)) = sol t"
+    using ODE_only_changes_not_zero_deriv[of x e d _ _ sol t] solx tv  by auto
+  ultimately show ?thesis by auto
+qed
+ 
+lemma diffE_aux: 
+  assumes "\<turnstile> {p}<odeone x e&&Inv&b>; DAss x e{b; H}"
+    and "DE_free e"
+    and "\<Turnstile> {p}<odeone x e&&Inv&b>; DAss x e{b; H}"
+  shows "\<Turnstile> {p}<odeone x e&&Inv&b>{b; H}"
+proof -
+  have "DE_free e \<Longrightarrow> semB (<odeone x e&&Inv&b>) now h now' h' \<Longrightarrow>
+    semB (<odeone x e&&Inv&b>; DAss x e) now h now' h'"
+    for now h now' h'
+  proof -
+    assume semode: "semB (<odeone x e&&Inv&b>) now h now' h'" and DEe: "DE_free e"
+    show "semB (<odeone x e&&Inv&b>; DAss x e) now h now' h'"
+    using semode DEe apply auto
+    subgoal for d sol 
+  proof -
+    assume de: "DE_free e"
+      and hi: "h' = (\<lambda>t. if t \<le> now + d \<and> now \<le> t then execute_ODE (odeone x e) (h now) (sol (t - now)) else h t)"
+      and d0: "0 \<le> d" and solx: "ODE_solution (odeone x e) d (h now) sol"
+      and dom: "\<forall>t. 0 \<le> t \<and> t < d \<longrightarrow> b (execute_ODE (odeone x e) (h now) (sol t))"
+      and dom2: "\<not> b (execute_ODE (odeone x e) (h now) (sol d))" and nowd: "now' = now + d"
+    show "semB (<odeone x e&&Inv&b>; DAss x e) now h (now + d) (\<lambda>t. if t \<le> now + d \<and> now \<le> t 
+      then execute_ODE (odeone x e) (h now) (sol (t - now)) else h t)"
+    proof -
+      have nowode: "now \<le> now'" using nowd d0 by auto
+      have ex: "evalE e (execute_ODE (odeone x e) (h now) (sol (now' - now))) =
+            snd (execute_ODE (odeone x e) (h now) (sol (now' - now))) $ x"
+        using diffE_lemma[of e x d _ _ sol "now'-now"] de solx nowd nowode
+        by (metis add.commute add_left_cancel d0 diff_add_cancel order_refl prod.exhaust_sel)
+      from ex have "update_snd (h' now') x (evalE e (h' now')) =  h' now'"
+        using nowode hi nowd
+        apply auto
+        by (smt eq_snd_iff fst_conv vec_lambda_unique)        
+      then have "h' = (\<lambda>t. if t = now' then update_snd (h' t) x (evalE e (h' t)) else h' t)"
+        by auto 
+      then have dasem: "semB (DAss x e) now' h' now' h'" 
+        using DassignB[of x e now' h'] by auto
+      then have "semB (<odeone x e&&Inv&b>) now h now' h' \<Longrightarrow> semB (DAss x e) now' h' now' h'"
+        by auto
+      then show ?thesis using sequenceB[of "<odeone x e&&Inv&b>" now h now' h' "DAss x e" now' h'] 
+        hi nowd semode by auto      
+    qed
+  qed
+  done
+  qed
+  then show ?thesis using assms unfolding Valid_def
+    by meson
+qed 
+
+lemma diffE2_aux: 
+  assumes "\<turnstile> {p}<odeone x e&&Inv&b>{b; H}"
+    and "DE_free e"
+    and "\<Turnstile> {p}<odeone x e&&Inv&b>{b; H}"
+  shows "\<Turnstile> {p}<odeone x e&&Inv&b>; DAss x e{b; H}"
+proof -
+  
+  have "DE_free e \<Longrightarrow> semB (<odeone x e&&Inv&b>; DAss x e) now h now' h' \<Longrightarrow>
+    semB (<odeone x e&&Inv&b>) now h now' h'"
+    for now h now' h'
+    apply auto
+    using if_split
+    sorry
+  then show ?thesis sorry
+qed
+
+
+lemma diffInvGE_aux: 
+  assumes "\<forall>s. b s \<longrightarrow> q s"
+    and "\<turnstile> {p}<odeone x e&&Inv&b>{Diff f1 [\<ge>] Diff f2; almost (Diff f1 [\<ge>] Diff f2) [[|]] elE 0}"
+    and "\<forall>h now now'. (almost (f1 [\<ge>] f2) [[|]] elE 0) h now now' \<longrightarrow> H h now now'"
+    and "well_DC H" 
+    and "\<Turnstile> {p}<odeone x e&&Inv&b>{Diff f1 [\<ge>] Diff f2; almost (Diff f1 [\<ge>] Diff f2) [[|]] elE 0}"
+  shows "\<Turnstile> {p}<odeone x e&&Inv&b>{f1 [\<ge>] f2; H}"
+  sorry
+
+lemma diffInvG_aux: 
+  assumes "\<forall>s. b s \<longrightarrow> q s"
+    and "\<turnstile> {p}<odeone x e&&Inv&b>{Diff f1 [>] Diff f2; almost (Diff f1 [>] Diff f2) [[|]] elE 0}"
+    and "\<forall>h now now'. (almost (f1 [>] f2) [[|]] elE 0) h now now' \<longrightarrow> H h now now'"
+    and "well_DC H" 
+    and "\<Turnstile> {p}<odeone x e&&Inv&b>{Diff f1 [>] Diff f2; almost (Diff f1 [>] Diff f2) [[|]] elE 0}"
+  shows "\<Turnstile> {p}<odeone x e&&Inv&b>{f1 [>] f2; H}"
+  sorry
+
+lemma diffGhost_aux:
+  assumes "\<forall>s. b s \<longrightarrow> q s"
+    and "\<turnstile> {p}<odeone x e&&Inv&b>{q; almost q [[|]] elE 0}"
+    and "\<forall>h now now'. (almost q [[|]] elE 0) h now now' \<longrightarrow> H h now now'"
+    and "well_DC H"
+    and "\<Turnstile> {p}<odeone x e&&Inv&b>{q; almost q [[|]] elE 0}"
+  shows "\<Turnstile> {p}<odeone x e&&Inv&b>{q; H}"
+  sorry
+
+
+
+theorem HHL_partial_sound : 
+  "\<turnstile> {p} P {q; H} \<Longrightarrow> \<Turnstile> {p} P {q; H}"
+proof (induction rule: HHL_partial.induct)
+  case (skipR p q H)
+  then show ?case 
+    apply (simp add:Valid_def, auto)
+    by (metis surj_pair)
+
+next
+  case (assignR p q x e H)
+  then show ?case
+    apply (simp add:Valid_def, auto)
+    by (metis (no_types, lifting) Cart_lambda_cong eq_snd_iff)
+
+next
+  case (seqR p P m H Q q G M)
+   then have "\<Turnstile> {p} P;  Q {q; H [^] G} \<and> (\<forall>h m n. (H[^]G) h m n \<longrightarrow> M h m n) " 
+     using Sequential_aux hhl_well_DC by blast
+   then show ?case unfolding Valid_def by auto 
+
+next
+  case (condTR p b P q H)
+  then show ?case
+    unfolding Valid_def 
+    using condTR.IH 
+    apply blast
+    done
+  next
+  case (condFR p q b H P)
+  then show ?case 
+    unfolding Valid_def
+    apply auto
+    apply (simp add: condFR.hyps)+
+    done 
+     
+next
+  case (IChoiceR p P m H Q q G)
+  then show ?case
+    unfolding Valid_def dOr_def fOr_def
+    by auto
+
+next
+  case (repetR H I P)
+  then show ?case 
+    unfolding Valid_def 
+    apply clarify
+    using repetitionN_sound[of H I P] 
+    by metis
+
+next
+  case (consequenceR px P qx Hx p q H)
+  then show ?case
+    unfolding Valid_def
+    apply auto
+    using consequenceR.hyps(2) consequenceR.hyps(3) apply blast
+    using consequenceR.hyps(2) consequenceR.hyps(3) apply blast
+    done
+
+next
+  case (continTR Inv b q p ode H)
+  show ?case 
+    unfolding Valid_def
+    apply auto
+    subgoal for now h d sol
+    proof -
+      assume d: "0 \<le> d" and s: "ODE_solution ode d (h now) sol" and 
+        dom: "\<forall>t. 0 \<le> t \<and> t < d \<longrightarrow> 
+          b (execute_ODE ode (h now) (sol t))" and dom2: " \<not> b (execute_ODE ode (h now) (sol d))"
+       and prep: "p (h now)" 
+      show "q (execute_ODE ode (h now) (sol d))"  
+      proof -
+        define S where "S = (execute_ODE ode (h now) (sol d))"
+        have "Inv S" using continTR.hyps(2) prep dom dom2 s d
+          unfolding ODE_inv_in_dom_def Let_def
+          using S_def by blast
+        moreover have "([\<not>] b) S" using dom dom2
+          unfolding fNot_def S_def Let_def by auto
+        ultimately show ?thesis using continTR.hyps(1) 
+          unfolding fAnd_def S_def by blast
+      qed
+    qed
+    subgoal for now h d sol
+    proof -
+      assume d: "0 \<le> d" and s: "ODE_solution ode d (h now) sol" and
+        dom: "\<forall>t. 0 \<le> t \<and> t < d \<longrightarrow> 
+          b (execute_ODE ode (h now) (sol t))" and dom2: "\<not> b (execute_ODE ode (h now) (sol d))"
+       and prep: "p (h now)"
+      show "H (\<lambda>t. if t \<le> now + d \<and> now \<le> t then execute_ODE ode (h now) (sol (t - now)) else h t) now (now + d)"
+     proof -
+       define P where "P = (\<lambda>t. if t \<le> now + d \<and> now \<le> t then 
+          execute_ODE ode (h now) (sol (t - now)) else h t)"
+       have "(almost (Inv [&] b) [[|]] elE 0) P now (now + d)"
+         unfolding dOr_def almost_def fAnd_def elE_def
+         apply auto
+         using d apply auto
+         prefer 2
+         using dom unfolding P_def Let_def
+          apply simp
+         using dom dom2 s continTR.hyps(2) prep d unfolding ODE_inv_in_dom_def Let_def 
+         apply auto
+         using d by (smt prod.collapse)
+       then show ?thesis using continTR.hyps(3) using P_def by auto
+     qed
+   qed
+   done
+ 
+next
+  case (diffCut p ode Inv b I q H)
+  then show ?case using diffCut_aux by auto
+
+next
+  case (diffWeak b H p ode Inv)
+  then show ?case
+    unfolding Valid_def
+    apply auto
+    unfolding fNot_def Let_def
+     apply blast
+    unfolding dOr_def by smt
+ 
+next
+  case (diffE p x e Inv b H)
+  then show ?case using diffE_aux by blast
+next
+  case (diffE2 p x e Inv b H)
+  then show ?case using diffE2_aux by blast
+next
+  case (diffInvGE b q p x e Inv f1 f2 H)
+  then show ?case using diffInvGE_aux by blast
+next
+  case (diffInvG b q p x e Inv f1 f2 H)
+  then show ?case using diffInvG_aux by blast
+next
+  case (diffGhost b q p x e Inv H)
+  then show ?case using diffGhost_aux by blast
+ 
+next
+  case (caseR p pb P q H)
+  then show ?case
+    unfolding Valid_def fNot_def fAnd_def
+    apply auto
+    apply blast
+    apply blast
+    done
+qed 
+
+lemma communication_aux:
+  assumes PQ: "\<turnstile> {px, py}P || Q{qx, qy; Hx, Hy}"
+    and postx: "\<forall>s. qx s \<longrightarrow> rx (update_fst s x (evalE e s))"
+    and posty: "\<forall>s. qy s \<longrightarrow> ry s"
+    and postHx: "\<forall>h n m. (Hx [^] (elE 0 [[|]] almost qx)) h n m \<longrightarrow> Gx h n m"
+    and postHy: "\<forall>h n m. (Hy [^] (elE 0 [[|]] almost qy)) h n m \<longrightarrow> Gy h n m"
+    and vPQ: "\<forall>nowp nowq fp fq nowp' nowq' fp' fq'.
+          semBP (P || Q) nowp fp nowq fq nowp' fp' nowq' fq' \<longrightarrow> px (fp nowp) \<longrightarrow> py (fq nowq) \<longrightarrow>
+           qx (fp' nowp') \<and> qy (fq' nowq') \<and> Hx fp' nowp nowp' \<and> Hy fq' nowq nowq'"
+  shows "semBP (P; Cm (ch[?]x) || Q; Cm (ch[!]e)) nowp fp nowq fq nowp' fp' nowq' fq' \<Longrightarrow>
+        px (fp nowp) \<Longrightarrow> py (fq nowq) \<Longrightarrow> 
+        rx (fp' nowp') \<and> ry (fq' nowq') \<and> Gx fp' nowp nowp' \<and> Gy fq' nowq nowq'"
+apply (ind_cases "semBP (P; Cm (ch[?]x) || Q; Cm (ch[!]e)) nowp fp nowq fq nowp' fp' nowq' fq'")
 apply (simp add:chanset_def) 
-apply (simp add:chanset_def) 
-apply (subgoal_tac " qx (fp'a nowp'a) \<and> qy (fq'a nowq'a) \<and> Hx fp'a nowp nowp'a \<and> Hy fq'a nowq nowq'a")
-prefer 2
-apply metis
-apply (rule conjI) 
-apply (subgoal_tac "fp' nowp' = (\<lambda> y. if y = x then evalE e (fp'a nowp'a) else (fp'a nowp'a) y)", simp)
-apply (metis less_irrefl)
-apply (rule conjI)
-apply (metis max.cobounded1 max_def_raw not_less)
-apply (rule conjI)
-(*to prove GX*)
-apply (subgoal_tac "(Hx[^](elE 0 [[|]] almost qx)) fp' nowp nowp'", simp)
-apply (subgoal_tac "Hx fp' nowp nowp'a",simp)
-prefer 2 
-apply (subgoal_tac "Hx fp'a nowp nowp'a = Hx fp' nowp nowp'a", simp)
-apply (smt DC semB1) 
-apply (smt almostint chop_def dOr_def semB1)
-(*to prove Gy, just copy the proof for Gx with a little adaption*)
-apply (subgoal_tac "(Hy[^](elE 0 [[|]] almost qy)) fq' nowq nowq'", simp)
-apply (subgoal_tac "Hy fq' nowq nowq'a",simp)
-prefer 2 
-apply (subgoal_tac "Hy fq'a nowq nowq'a = Hy fq' nowq nowq'a", simp)
-apply (smt DC semB1)
-by (smt almostint chop_def dOr_def semB1)
+apply (simp add:chanset_def)
+  subgoal for nowp'a fp'a nowq'a fq'a
+  proof -
+    assume 1: "px (fp nowp)" and 2: "py (fq nowq)" and 3: "nowp' = max nowp'a nowq'a"
+      and 4: "fp' = (\<lambda>t. if nowp'a < t \<and> t < max nowp'a nowq'a then fp'a nowp'a
+         else if t = max nowp'a nowq'a then update_fst (fp'a nowp'a) x (evalE e (fp'a nowp'a)) else fp'a t)"
+      and 5: "nowq' = max nowp'a nowq'a" 
+      and 6: "fq' = (\<lambda>t. if nowq'a < t \<and> t \<le> max nowp'a nowq'a then fq'a nowq'a else fq'a t)"
+      and 7: "semBP (P || Q) nowp fp nowq fq nowp'a fp'a nowq'a fq'a" and 8: "ch = ch"
+    show "rx (fp' nowp') \<and> ry (fq' nowq') \<and> Gx fp' nowp nowp' \<and> Gy fq' nowq nowq'"
+    proof -
+      have postPQ: "qx (fp'a nowp'a) \<and> qy (fq'a nowq'a) \<and> Hx fp'a nowp nowp'a \<and> Hy fq'a nowq nowq'a"
+        using 7 PQ vPQ 1 2 by auto
+      then have postp: "rx (fp' nowp')" using 3 4 postx by fastforce
+      have postq: "ry (fq' nowq')" using postPQ 5 6 posty  
+        by (simp add: posty max.strict_order_iff)
+      have "Hx fp' nowp nowp'a" using postPQ semB1[of P Q nowp fp nowq fq nowp'a fp'a nowq'a fq'a] 
+        hhl_well_DC_par[of px py P Q qx qy Hx Hy] PQ 4 7
+        unfolding well_DC_def by smt
+      moreover have "(elE 0 [[|]] almost qx) fp' nowp'a nowp'"
+        unfolding chop_def almost_def dOr_def elE_def 4 3 
+        using postPQ by auto
+      ultimately have postpH: "(Hx [^] (elE 0 [[|]] almost qx)) fp' nowp nowp'"
+        unfolding chop_def using 3 
+        by (meson "7" max.cobounded1 semB1)
 
-lemma CommunicationRule : 
-  " ({px, py} (P || Q) {qx, qy; Hx, Hy}) \<Longrightarrow>  
-   (\<forall> s. qx s \<longrightarrow> (rx (% y. if (y=x) then (evalE e s) else s y)))
- \<and> (\<forall> s. qy s \<longrightarrow> ry s)
- \<and> (\<forall> h n m. (Hx[^](elE 0 [[|]]almost qx)) h n m \<longrightarrow> Gx h n m) \<and> 
-   (\<forall> h n m. (Hy[^](elE 0 [[|]]almost qy)) h n m \<longrightarrow> Gy h n m)
-  ==>
-{px, py} (P;Cm (ch??(RVar (x))))||(Q; (Cm (ch!!e))) {rx, ry; Gx, Gy}"
-  apply (clarsimp simp:ValidP_def) 
-  apply (cut_tac P = P and Q = Q and ch = ch and px = px and py = py and rx = rx and ry = ry and
-    Gx = Gx and Gy = Gy in Communication_aux, auto)
-  done  
+      have "Hy fq' nowq nowq'a" using postPQ semB1[of P Q nowp fp nowq fq nowp'a fp'a nowq'a fq'a] 
+        hhl_well_DC_par[of px py P Q qx qy Hx Hy] PQ 6 7
+        unfolding well_DC_def by smt
+      moreover have "(elE 0 [[|]] almost qy) fq' nowq'a nowq'"
+        unfolding chop_def almost_def dOr_def elE_def 5 6
+        using postPQ by auto
+      ultimately have postqH: "(Hy [^] (elE 0 [[|]] almost qy)) fq' nowq nowq'"
+        unfolding chop_def using 5 
+        by (meson "7" max.cobounded2 semB1)
 
-(*Parallel rule for the case with non-communication process at the end.*)
-lemma Parallel2_aux : "semBP (P; U || Q; V) nowp fp nowq fq nowp' fp' nowq' fq' \<Longrightarrow>
-        \<forall>nowp nowq fp fq nowp' nowq' fp' fq'.
-          semBP (P || Q) nowp fp nowq fq nowp' fp' nowq' fq' \<longrightarrow>
-          pp (fp nowp) \<longrightarrow> pq (fq nowq) \<longrightarrow> qp (fp' nowp') \<and> qq (fq' nowq') \<and> 
-        Hp fp' nowp nowp' \<and> Hq fq' nowq nowq' \<Longrightarrow>
-       \<forall>now h now' h'. semB U now h now' h' \<longrightarrow> qp (h now) \<longrightarrow> qu (h' now') \<and> Hu h' now now' \<Longrightarrow>
-       \<forall>now h now' h'. semB V now h now' h' \<longrightarrow> qq (h now) \<longrightarrow> qv (h' now') \<and> Hv h' now now' \<Longrightarrow>
-       chanset P \<noteq> {} \<Longrightarrow> chanset Q \<noteq> {} \<Longrightarrow> chanset U = {} \<Longrightarrow> chanset V = {} \<Longrightarrow>
-       pp (fp nowp) \<Longrightarrow> pq (fq nowq) \<Longrightarrow> qu (fp' nowp') \<and> qv (fq' nowq') \<and> 
-             (Hp[^]Hu) fp' nowp nowp' \<and> (Hq[^]Hv) fq' nowq nowq'"
+      from postp postq postpH postqH postHx postHy show ?thesis by auto
+    qed
+  qed
+  done
+  
+
+lemma parallel_aux: 
+  " \<turnstile> {pp, pq}P || Q{qp, qq; Hp, Hq} \<Longrightarrow>
+       \<turnstile> {qp}U{qu; Hu} \<Longrightarrow>
+       \<turnstile> {qq}V{qv; Hv} \<Longrightarrow>
+       \<forall>nowp nowq fp fq nowp' nowq' fp' fq'.
+          semBP (P || Q) nowp fp nowq fq nowp' fp' nowq' fq' \<longrightarrow> pp (fp nowp) \<longrightarrow> pq (fq nowq) \<longrightarrow>
+          qp (fp' nowp') \<and> qq (fq' nowq') \<and> Hp fp' nowp nowp' \<and> Hq fq' nowq nowq' \<Longrightarrow>
+       chanset P \<noteq> {} \<Longrightarrow>
+       chanset Q \<noteq> {} \<Longrightarrow>
+       chanset U = {} \<Longrightarrow>
+       chanset V = {} \<Longrightarrow>
+       semBP (P; U || Q; V) nowp fp nowq fq nowp' fp' nowq' fq' \<Longrightarrow>
+       pp (fp nowp) \<Longrightarrow> pq (fq nowq) \<Longrightarrow> 
+       qu (fp' nowp') \<and> qv (fq' nowq') \<and> (Hp [^] Hu) fp' nowp nowp' \<and> (Hq [^] Hv) fq' nowq nowq'"
 apply (ind_cases "semBP (P; U || Q; V) nowp fp nowq fq nowp' fp' nowq' fq'")
 apply (simp add:chanset_def)
 prefer 2 apply (simp add:chanset_def)
 prefer 2 apply (simp add:chanset_def)
-apply (subgoal_tac "qp (fp'a nowp'a) \<and> qq (fq'a nowq'a) \<and> Hp fp'a nowp nowp'a \<and> Hq fq'a nowq nowq'a")
-prefer 2
-apply metis
-apply (rule conjI) apply metis
-apply (rule conjI) apply metis
-apply (subgoal_tac "(Hu) fp' nowp'a nowp' ")
-apply (subgoal_tac "(Hv) fq' nowq'a nowq'")
-prefer 2 apply metis prefer 2 apply metis
-apply (subgoal_tac " Hq fq' nowq nowq'a")
-apply (subgoal_tac " Hp fp' nowp nowp'a ")
-apply (rule conjI)
-apply (unfold chop_def)
-apply (metis sem1 semB1)
-apply (metis sem1 semB1)
-apply (subgoal_tac "Hp fp'a nowp nowp'a = Hp fp' nowp nowp'a", simp)
-apply (smt DC sem2 semB1) 
-apply (subgoal_tac " Hq fq'a nowq nowq'a =  Hq fq' nowq nowq'a", simp) 
-by (smt DC sem2 semB1)
+  subgoal for nowp'a fp'a nowq'a fq'a 
+  proof -
+    assume 1: "\<turnstile> {pp, pq}P || Q{qp, qq; Hp, Hq}"
+      and 2: "\<turnstile> {qp}U{qu; Hu}" and 3: "\<turnstile> {qq}V{qv; Hv}"
+      and 4: "\<forall>nowp nowq fp fq nowp' nowq' fp' fq'.  
+           semBP (P || Q) nowp fp nowq fq nowp' fp' nowq' fq' \<longrightarrow> pp (fp nowp) \<longrightarrow> pq (fq nowq) \<longrightarrow>
+            qp (fp' nowp') \<and> qq (fq' nowq') \<and> Hp fp' nowp nowp' \<and> Hq fq' nowq nowq'"
+      and 5: "chanset P \<noteq> {}" and 6: "chanset Q \<noteq> {}" and 7: "chanset U = {}" and 8: "chanset V = {}"
+      and 9: "pp (fp nowp)" and 10: "pq (fq nowq)"
+      and 11: "semBP (P || Q) nowp fp nowq fq nowp'a fp'a nowq'a fq'a"
+      and 12: "semB U nowp'a fp'a nowp' fp'" and 13: "semB V nowq'a fq'a nowq' fq'"
+    and "chanset P \<noteq> {}" and "chanset Q \<noteq> {}" and "chanset U = {}" and "chanset V = {}"  
+     show "qu (fp' nowp') \<and> qv (fq' nowq') \<and> (Hp [^] Hu) fp' nowp nowp' \<and> (Hq [^] Hv) fq' nowq nowq'"
+     proof -
+       have wpq: "qp (fp'a nowp'a) \<and> qq (fq'a nowq'a) \<and> Hp fp'a nowp nowp'a \<and> Hq fq'a nowq nowq'a"
+         using 4 11 9 10 by auto
+       moreover have "\<Turnstile> {qp}U{qu; Hu} \<and> \<Turnstile> {qq}V{qv; Hv}"
+         using 2 3 HHL_partial_sound by auto
+       ultimately have wuv: "qu (fp' nowp') \<and> qv (fq' nowq') \<and> Hu fp' nowp'a nowp' \<and> Hv fq' nowq'a nowq'" 
+         unfolding Valid_def using 12 13 by auto
 
-
-lemma Parallel2Rule : "{pp, pq} P||Q {qp, qq; Hp, Hq}  \<Longrightarrow> chanset P \<noteq> {} \<and> chanset Q \<noteq> {} \<Longrightarrow> 
-                          {qp} U {qu; Hu} \<Longrightarrow> {qq} V {qv; Hv} \<Longrightarrow> chanset U = {} \<and> chanset V = {} 
-                       \<Longrightarrow> {pp, pq} P; U||Q; V {qu, qv; Hp [^] Hu, Hq [^] Hv}"
-apply (clarsimp simp:Valid_def ValidP_def)
-apply (rule Parallel2_aux)
-apply simp+
-done
+       have "Hp fp' nowp nowp'a \<and> Hq fq' nowq nowq'a"
+         using wpq sem2 well_DC_def[of Hp] hhl_well_DC_par[of pp pq P Q qp qq Hp Hq] 1
+           well_DC_def[of Hq] semB1 semB2
+         by (smt "11" "12" "13")
+       then show ?thesis unfolding chop_def using wpq wuv
+         by (meson "11" "12" "13" sem1 semB1)
+     qed
+   qed
+   done
  
-(*Repetition rule*)
-  
-  
-lemma Repetition_aux_1: " semB (P* NUM 0) now h now' h' \<Longrightarrow>
-       \<forall>h n m. (H[^]H) h n m \<longrightarrow> H h n m \<Longrightarrow>
-       \<forall>now h now' h'. semB P now h now' h' \<longrightarrow> Inv (h now) \<longrightarrow> Inv (h' now') \<and> H h' now now' \<Longrightarrow>
-       Inv (h now) \<Longrightarrow> Inv (h' now') \<and> (H h' now now' \<or> now' = now)"
-  apply (ind_cases "semB (P* NUM 0) now h now' h'", auto)
-  done
-    
-    
-lemma Repetition_aux_2: " (\<And>now h now' h'. semB (P* NUM N) now h now' h' \<Longrightarrow> Inv (h now) \<Longrightarrow> Inv (h' now') \<and> (H h' now now' \<or> now' = now)) \<Longrightarrow>
-       semB (P* NUM Suc N) now h now' h' \<Longrightarrow>
-       \<forall>h n m. (H[^]H) h n m \<longrightarrow> H h n m \<Longrightarrow>
-       \<forall>now h now' h'. semB P now h now' h' \<longrightarrow> Inv (h now) \<longrightarrow> Inv (h' now') \<and> H h' now now' \<Longrightarrow>
-       Inv (h now) \<Longrightarrow> Inv (h' now') \<and> (H h' now now' \<or> now' = now)"
-  apply (ind_cases "semB (P* NUM Suc N) now h now' h'")
-  apply simp
-  by (smt DC chop_def sem1 sem2)
 
-lemma Repetition_aux: "semB (P* NUM N) now h now' h' \<Longrightarrow> 
-                     \<forall>h n m. (H[^]H) h n m \<longrightarrow> H h n m \<Longrightarrow>
-                     \<forall>now h now' h'. semB P now h now' h' \<longrightarrow> Inv (h now) \<longrightarrow> Inv (h' now') \<and> H h' now now' \<Longrightarrow>
-                     Inv (h now) \<Longrightarrow> Inv (h' now') \<and> (H [[|]] (\<lambda>h n nd. nd = n)) h' now now'"
-apply (simp add:dOr_def)
-apply (induction N arbitrary: now h now' h')
-apply (cut_tac H = H and P = P and now = now and h = h and now' = now' and h' = h' in Repetition_aux_1) 
-apply simp+
-apply (cut_tac P = P and N = N and now = now and h = h and h' = h' and Inv = Inv in Repetition_aux_2, auto)
-done
-
-lemma RepetitionRule: "\<forall>h n m. (H[^]H) h n m \<longrightarrow> H h n m \<Longrightarrow> {I} P {I; H}  
-                      ==>  {I} P*&&I {I; (H [[|]] (elE 0))} "
-  apply (simp add:Valid_def) apply clarify 
-  apply (rule Repetition_aux)
-   apply simp+
+theorem HHL_para_sound : 
+  "\<turnstile> {pp, pq} P||Q {qp, qq; Hp, Hq} \<Longrightarrow>  \<Turnstile> {pp, pq} P||Q {qp, qq; Hp, Hq}" 
+proof (induction rule: HHL_para.induct)
+  case (parallelR P Q pp qp Hp pq qq Hq)
+  then have chs: "chanset P = {} \<and> chanset Q = {}"
+    and vP: "\<Turnstile> {pp} P {qp; Hp}" and vQ: "\<Turnstile> {pq} Q {qq; Hq}"
+    using HHL_partial_sound by auto
+  show ?case
+    unfolding ValidP_def
+    apply clarify
+    subgoal for nowp nowq fp fq nowp' nowq' fp' fq' 
+    proof -
+      assume PQ: "semBP (P || Q) nowp fp nowq fq nowp' fp' nowq' fq'" and 
+             preP: "pp (fp nowp)" and preQ: "pq (fq nowq)"
+      show "qp (fp' nowp') \<and> qq (fq' nowq') \<and> Hp fp' nowp nowp' \<and> Hq fq' nowq nowq'"
+      proof -
+        have "semB P nowp fp nowp' fp' \<and> semB Q nowq fq nowq' fq'"
+          using PQ semB3 chs by metis
+        then show ?thesis using vP vQ preP preQ unfolding Valid_def by metis
+      qed
+    qed
   done
 
-   
-lemma JoinRule : "{p} P {m; H} \<Longrightarrow> {p} Q {q; G} ==>
-             {p} P [[ Q {m [|] q; H [[|]] G}"
-  apply (simp add:Valid_def fOr_def dOr_def, auto)
-    done
+next
+  case (commR px py P Q qx qy Hx Hy rx x e ry Gx Gy ch)
+  then show ?case
+    unfolding ValidP_def
+    apply clarify
+    using communication_aux[of px py P Q qx qy Hx Hy rx x e ry Gx Gy ch]
+    by presburger 
 
-
-
-(*Consequence rule*)
-lemma ConsequenceRule : "{px} P {qx; Hx} 
-                  \<and> (\<forall> s. p s \<longrightarrow> px s) \<and> (\<forall> s. qx s \<longrightarrow> q s)
-                  \<and> (\<forall> h n m. Hx h n m \<longrightarrow> H h n m)
-            ==> {p} P {q; H}"
-apply (simp add:Valid_def)
-done
-
-lemma RepetitionRule_a :  "\<forall>h n m. (H[^]H) h n m \<longrightarrow> H h n m \<Longrightarrow> {I} P {I; H}  
-                      ==>  {I} P*&&I {I; ((elE 0) [[|]] H)} "
-                      apply (cut_tac px = "I" and qx = I and Hx = "(H [[|]] (elE 0))" in ConsequenceRule, auto)
-                      apply (cut_tac RepetitionRule, auto)
-                      using dOr_def by auto
+next
+  case (parallel2R pp pq P Q qp qq Hp Hq U qu Hu V qv Hv)
+  then show ?case 
+    unfolding ValidP_def
+    apply clarify 
+    using parallel_aux[of pp pq P Q qp qq Hp Hq U qu Hu V qv Hv]
+    by presburger
+qed
  
-(*Case analysis rule*)
-lemma CaseRule : "{p [&] pb} P {q; H} \<and> {(p [&] ([\<not>]pb))} P {q; H}
-   ==> {p} P {q; H}"
-apply (simp add:Valid_def fAnd_def fNot_def, auto)
-apply metis+
-done
-
+declare almost_def [simp del]
+declare chop_def [simp del]
+ 
+ 
 end
