lunarlander/Op_SL.thy
@@ -1,21 +1,24 @@
 section \<open>Operation semantics of HCSP.\<close>
 
 theory Op_SL
-  imports State_SL
+  imports Syntax_SL
 begin
+
+type_synonym now = real
+type_synonym 'a history = "time \<Rightarrow> 'a pair_state"
+
+definition semf :: "'a pair_state \<Rightarrow> 'a fform \<Rightarrow> bool" ("_ |= _" 50) where
+  "semf s f \<equiv> f s"
 
 text \<open>Five kinds of events for HCSP processes\<close>
 datatype event = Tau | In cname real | Out cname real | IO cname real | Delay time
-type_synonym now = real
-
+ 
+ 
 text \<open>Continuous evolution\<close>
+  
 
-datatype flow = Flow "string list" "exp list"
-text \<open>Explicit solution\<close>
-consts Solution :: "flow \<Rightarrow> state \<Rightarrow> real \<Rightarrow> real"
-
-consts evalP :: "proc \<Rightarrow> now \<Rightarrow> history \<Rightarrow> event * proc * now * history"
-consts evalPP :: "procP \<Rightarrow> now \<Rightarrow> history \<Rightarrow> history \<Rightarrow> event * procP * now * history * history"
+consts evalP :: "'a proc \<Rightarrow> now \<Rightarrow> 'a history \<Rightarrow> event * 'a proc * now * 'a history"
+consts evalPP :: "'a procP \<Rightarrow> now \<Rightarrow> 'a history \<Rightarrow> 'a history \<Rightarrow> event * 'a procP * now * 'a history * 'a history"
 
  
 text \<open>Parallel composition\<close>
@@ -37,64 +40,134 @@ primrec handshake :: "event \<Rightarrow> event \<Rightarrow> event" where
 | "handshake (Delay d) ev = Tau"
 
 text \<open>Set of channels of a procedure\<close>
-primrec chansetC :: "comm => string set" where 
-  "chansetC (ch!!e) = {ch}"
-| "chansetC (ch??e) = {ch}"
+primrec chansetC :: "'a comm => string set" where 
+  "chansetC (ch[!]e) = {ch}"
+| "chansetC (ch[?]e) = {ch}"
                             
-primrec chanset :: "proc \<Rightarrow> string set" where
+primrec chanset :: "'a proc \<Rightarrow> string set" where
   "chanset (Cm r) = chansetC r"
 | "chanset Skip = {}"
 | "chanset (e := f) = {}"
 | "chanset (P; Q) = chanset P \<union> chanset Q"
 | "chanset (IF b P) = chanset P"
-| "chanset (C \<rightarrow> P) = chansetC C \<union> chanset P"
-| "chanset (P [[ Q) = chanset P \<union> chanset Q"
-| "chanset (P << Q) = chanset P \<union> chanset Q"
-  (*"chanset (P || Q) = chanset P \<union> chanset Q" |*)
+| "chanset (P \<sqinter> Q) = chanset P \<union> chanset Q"
+| "chanset (c \<rightarrow> P [] d \<rightarrow> Q) = chansetC c  \<union> chansetC d  \<union> chanset P \<union> chanset Q"
 | "chanset (P *&& Inv) = chanset P"
-| "chanset (<vl : el && Inv & b>) = {}"
-| "chanset (P [[> Q) = chanset P \<union> chanset Q"
+| "chanset (P * NUM n) = chanset P"
+| "chanset (<ODEs && Inv & b>) = {}"
+| "chanset (P []c \<rightarrow> Q) = chanset P \<union> chanset Q \<union> chansetC c"
+
+text \<open>Definitions for ODEs\<close>
+ 
+text \<open>The semantics of an ODE is the value of the vector field.\<close>
+fun ODE_sem :: "'a :: finite ODE \<Rightarrow> 'a state \<Rightarrow> 'a state" 
+  where
+  "ODE_sem (odeone x e) = (\<lambda> s. (\<chi> i. if i = x then (evalE_df e s) else 0))"
+| "ODE_sem (odes ode1, ode2)  = (\<lambda> s. ((ODE_sem ode1 s) + (ODE_sem ode2 s)))"
+  
+definition ODE_pair_state :: "'a :: finite ODE \<Rightarrow> 'a state \<Rightarrow> 'a pair_state"
+  where "ODE_pair_state ode u = (u, ODE_sem ode u)"
+ 
+definition execute_ODE :: "'a :: finite ODE \<Rightarrow> 'a pair_state \<Rightarrow> 'a state \<Rightarrow> 'a pair_state"
+  where "execute_ODE ode \<nu> u = 
+     (THE \<omega>. Vagree  \<omega> \<nu> (- ODE_vars ode) \<and> (Vagree \<omega> (ODE_pair_state ode u) (ODE_vars ode)))"
+
+text \<open>Construct a concrete solution for the ODE.\<close>
+definition concrete_sol :: "'a :: finite ODE \<Rightarrow> 'a pair_state \<Rightarrow> 'a state \<Rightarrow> 'a pair_state"
+  where "concrete_sol ode \<nu> u = 
+ ((\<chi> i. (if i \<in> ODE_vars ode then u else (fst \<nu>)) $ i), 
+  (\<chi> i. (if i \<in> ODE_vars ode then ODE_sem ode u else (snd \<nu>)) $ i))"
+
+lemma execute_ODE_exists: 
+  "\<exists> \<omega>. Vagree  \<omega> \<nu> (- ODE_vars ode) \<and> (Vagree \<omega> (ODE_pair_state ode u) (ODE_vars ode))"
+ by(rule exI[where x="(concrete_sol ode \<nu> u)"], auto simp add: concrete_sol_def ODE_pair_state_def Vagree_def)
+ 
+lemma execute_ODE_agree: "Vagree (execute_ODE ode \<nu> u) \<nu> (- ODE_vars ode)
+   \<and> Vagree (execute_ODE ode \<nu> u) (ODE_pair_state ode u) (ODE_vars ode)"
+   unfolding execute_ODE_def Let_def
+   apply (rule theI[where a = "concrete_sol ode \<nu> u"], auto)
+   apply (simp add:concrete_sol_def ODE_pair_state_def Vagree_def Let_def)+
+   using exE[OF execute_ODE_exists, of \<nu>  ode u]
+   by (auto simp add: concrete_sol_def ODE_pair_state_def Vagree_def vec_eq_iff)
+ 
+lemma execute_ODE_concrete: "execute_ODE ode \<nu> u = concrete_sol ode \<nu> u"
+  apply (simp add:concrete_sol_def)
+  apply(rule Vagree_eq)
+  using execute_ODE_agree[of ode \<nu> u]
+  unfolding Vagree_def ODE_pair_state_def by auto
+
+text \<open>The solution of ode at time interval {0..t} with respect to initial state \<nu>\<close>
+definition ODE_solution :: "'a :: finite ODE \<Rightarrow> real => 'a pair_state \<Rightarrow> (real \<Rightarrow> 'a state) \<Rightarrow> bool"
+  where "ODE_solution ode t \<nu> v = ((v has_vderiv_on (\<lambda>t. ODE_sem ode (v t))) {0..t} \<and> v 0 = fst \<nu>)" 
+
+definition ODE_solution_in_dom :: "'a :: finite ODE \<Rightarrow> real => 'a pair_state \<Rightarrow> 'a fform \<Rightarrow> (real \<Rightarrow> 'a state) \<Rightarrow> bool"
+  where "ODE_solution_in_dom ode t \<nu> b v  = ((v solves_ode (\<lambda>_. ODE_sem ode)) {0..t} {x. b (execute_ODE ode \<nu> x)} \<and> v 0 = fst \<nu>)"
+
+text \<open>\<nu> is the initial state, b is the domain, and i is the invariant\<close>
+definition ODE_inv_in_dom :: "'a :: finite ODE \<Rightarrow>'a pair_state \<Rightarrow> 'a fform \<Rightarrow> 'a fform \<Rightarrow> bool"
+  where "ODE_inv_in_dom ode \<nu> b i = (\<forall> d \<ge> 0. \<forall> sol. (ODE_solution ode d \<nu> sol --> 
+    ((\<forall> t. t \<ge> 0 \<and> t < d \<longrightarrow> b (execute_ODE ode \<nu> (sol t))) \<longrightarrow>
+    (\<forall> t. t \<ge> 0 \<and> t \<le> d \<longrightarrow> i (execute_ODE ode \<nu> (sol t))))))"
+(*  where "ODE_inv_in_dom ode d \<nu> b inv = (let sol = ODE_solution ode d \<nu> in 
+      (\<forall> t. t \<ge> 0 \<and> t < d \<longrightarrow> b (execute_ODE ode \<nu> (sol t))) \<longrightarrow> 
+      (\<forall> t. t \<ge> 0 \<and> t < d \<longrightarrow> inv (execute_ODE ode \<nu> (sol t))))"
+*)
+
+(*
+text \<open>With a change of differential variables in the second state\<close>
+definition the_first_state :: "'a :: finite ODE \<Rightarrow>'a pair_state \<Rightarrow> 'a pair_state"
+  where "the_first_state ode \<nu> = execute_ODE ode \<nu> (ODE_solution ode 0 \<nu> 0)"
+*)
+
+fun update_fst :: "'a :: finite pair_state \<Rightarrow> 'a \<Rightarrow> real \<Rightarrow> 'a pair_state" 
+  where "update_fst u a r = ((\<chi> i. if i = a then r else fst u $ i), snd u)"
+
+fun update_snd :: "'a :: finite pair_state \<Rightarrow> 'a \<Rightarrow> real \<Rightarrow> 'a pair_state" 
+  where "update_snd u a r = (fst u, (\<chi> i. if i = a then r else snd u $ i))"
+
+fun extend_history :: "'a :: finite history \<Rightarrow> real \<Rightarrow> real \<Rightarrow> 'a history"
+  where "extend_history f a d = (\<lambda> t. if t > a \<and> t \<le> a + d then f a else f t)"
 
 
 text \<open>Small step semantics for HCSP.\<close>
-
-inductive semP :: "proc \<Rightarrow> now \<Rightarrow> history \<Rightarrow> (event * proc * now * history) \<Rightarrow> bool" where
+inductive semP :: "'a :: finite proc \<Rightarrow> now \<Rightarrow> 'a history \<Rightarrow> (event * 'a proc * now * 'a history) \<Rightarrow> bool" where
   skip: "semP Skip now f (Tau, Skip, now, f)"
-| assignR: "semP ((RVar x) := e) now f
-    (Tau, Skip, now, (\<lambda>t. if t = now then (\<lambda> y. if y=x then evalE e (f t) else f t y) else f t))"
-| continuousF: "([\<not>]b) (f now) \<Longrightarrow>
-    semP (<[s]:E&&Inv&b>) now f (Tau, Skip, now, f)"
-| continuousT: "d\<ge>0 \<Longrightarrow>
-       let f' = (\<lambda>t. if t \<le> now+d \<and> t > now then
-                       (\<lambda> y. if y = s then Solution (Flow [s] E) (f now) (t-now) else f now y)
-                     else f t)
-       in \<forall>m. m \<le> now+d \<and> m \<ge> now \<longrightarrow> b (f' m) \<Longrightarrow>
-    semP (<[s]:E&&Inv&b>) now f
-      (Delay d, <[s]:E&&Inv&b>, now+d,
+| assign: "semP (x := e) now f
+    (Tau, Skip, now, (\<lambda>t. if t = now then (update_fst (f t) x (evalE e (f t))) else f t))"
+| Dassign: "semP (DAss x e) now f 
+    (Tau, Skip, now, (\<lambda>t. if t = now then (update_snd (f t) x (evalE e (f t)))  else f t))"
+| continuousF: "([\<not>]b) (execute_ODE ode (f now) (fst (f now))) \<Longrightarrow>
+    semP (<ode && Inv&b>) now f (Tau, Skip, now, (\<lambda>t. if t = now then (execute_ODE ode (f now) (fst (f now))) else f t))"
+| continuousT: "d > 0 \<Longrightarrow> ODE_solution_in_dom ode d (f now) b sol \<Longrightarrow>
+    semP (<ode && Inv&b>) now f (Delay d, <ode && Inv&b>, now+d,
        (\<lambda>t. if t \<le> now+d \<and> t > now then
-              (\<lambda> y. if y = s then Solution (Flow [s] E) (f now) (t-now) else f now y)
-            else f t))"
-| sequenceL: "semP P now f (ev, P', now', f') \<and> P'\<noteq>Skip \<Longrightarrow>
-              semP (P; Q) now f (ev, P';Q, now', f')"
-| sequenceR: "semP P now f (ev, P', now', f') \<and> P'=Skip \<Longrightarrow>
+              (execute_ODE ode (f now) (sol (t-now)))  else f t))"
+| sequenceL: "semP P now f (ev, P', now', f') \<and> P' \<noteq> Skip \<Longrightarrow>
+              semP (P; Q) now f (ev, P'; Q, now', f')"
+| sequenceR: "semP P now f (ev, P', now', f') \<and> P' = Skip \<Longrightarrow>
               semP (P; Q) now f (ev, Q, now', f')"
 | conditionT: " b (f now) \<Longrightarrow> semP (IF b P) now f (Tau, P, now, f)"
 | conditionF: "\<not>b (f now) \<Longrightarrow> semP (IF b P) now f (Tau, Skip, now, f)"
-| joinL: "semP (P[[Q) now f (Tau, P, now, f)"
-| joinR: "semP (P[[Q) now f (Tau, Q, now, f)"
-| repetition0: "semP (P*&&Inv) now f (Tau, Skip, now, f)"
-| repetitionk: "semP P now f (ev, P', now', f') \<and> P'\<noteq>Skip \<Longrightarrow>
-                semP (P*&&Inv) now f (ev, (P'; P*&&Inv), now', f')"
-| repetitionk1: "semP P now f (ev, P', now', f') \<and> P'=Skip \<Longrightarrow>
-                  semP (P*&&Inv) now f (ev, P*&&Inv, now',f')"
-| outputC : "semP (Cm (ch!!e)) now f (Out ch (evalE e (f now)), Skip, now, f)"
-| outputW : "d\<ge>0 \<Longrightarrow> semP (Cm (ch!!e)) now f
-            (Delay d, Cm (ch!!e), now+d, \<lambda>t. if t \<le> now+d \<and> t > now then f now else f t)"
-| inputC : "semP (Cm (ch??x)) now f (In ch c, x := (Real c), now, f)"
-| inputW : "d\<ge>0 \<Longrightarrow> semP (Cm (ch??x)) now f
-            (Delay d, Cm (ch??x), now+d, \<lambda>t. if t \<le> now+d \<and> t > now then f now else f t)"
+| IChoiceL: "semP (P \<sqinter> Q) now f (Tau, P, now, f)"
+| IChoiceR: "semP (P \<sqinter> Q) now f (Tau, Q, now, f)"
+| EChoiceL: "semP (ch [!] e \<rightarrow> P [] dh [?] x \<rightarrow> Q) now f (Out ch (evalE e (f now)), P, now, f)"
+| EChoiceR: "semP (ch [!] e \<rightarrow> P [] dh [?] x \<rightarrow> Q) now f (In dh c, (x := (Real c); P), now, f)"
+| EChoiceW: "d\<ge>0 \<Longrightarrow> semP (ch [!] e \<rightarrow> P [] dh [?] x \<rightarrow> Q) now f 
+              (Delay d, (ch [!] e \<rightarrow> P [] dh [?] x \<rightarrow> Q), now + d, extend_history f now d)"
+| repetition0: "semP (P *&& Inv) now f (Tau, Skip, now, f)"
+| repetitionk: "semP P now f (ev, P', now', f') \<and> P' \<noteq> Skip \<Longrightarrow>
+                semP (P *&& Inv) now f (ev, (P'; P *&& Inv), now', f')"
+| repetitionk1: "semP P now f (ev, P', now', f') \<and> P' = Skip \<Longrightarrow>
+                  semP (P *&& Inv) now f (ev, P *&& Inv, now',f')"
+| outputC : "semP (Cm (ch[!]e)) now f (Out ch (evalE e (f now)), Skip, now, f)"
+| outputW : "d\<ge>0 \<Longrightarrow> semP (Cm (ch[!]e)) now f
+            (Delay d, Cm (ch[!]e), now + d, extend_history f now d)"
+| inputC : "semP (Cm (ch[?]x)) now f (In ch c, x := (Real c), now, f)"
+| inputW : "d\<ge>0 \<Longrightarrow> semP (Cm (ch[?]x)) now f
+            (Delay d, Cm (ch[?]x), now + d, extend_history f now d)"
+ 
 
-inductive semPP :: "procP \<Rightarrow> now \<Rightarrow> history \<Rightarrow> history \<Rightarrow> (event * procP * now * history * history) \<Rightarrow> bool" where
+inductive semPP :: "'a :: finite procP \<Rightarrow> now \<Rightarrow> 'a history \<Rightarrow> 'a history \<Rightarrow> (event * 'a procP * now * 'a history * 'a history) \<Rightarrow> bool" where
   parallel0: "semPP (P||Q) now f g (eve, P'||Q', now', f', g') \<Longrightarrow> semPP (Q||P) now g f (eve, Q'||P', now', g', f')"
 | parallel1: "semP P now f (evp, P', now, f') \<and> semP Q now g (evq, Q', now, g') \<and> compat evp evq \<Longrightarrow>
               semPP (P||Q) now f g (handshake evp evq, P'||Q', now, f', g')"
@@ -104,93 +177,85 @@ inductive semPP :: "procP \<Rightarrow> now \<Rightarrow> history \<Rightarrow> 
                 (\<exists>ch c. evp = In ch c \<and> \<not>(ch \<in> chanset P \<inter> chanset Q)) \<or>
                 (\<exists>ch c. evp = IO ch c \<and> \<not>(ch \<in> chanset P \<inter> chanset Q))) \<Longrightarrow>
              semPP (P||Q) now f g (evp, P'||Q, now', f', g)"
-| parallel3 : "semP P now f (Delay d, P', now+d, f')
-              \<and> semP Q now g (Delay d, Q', now+d, g') \<Longrightarrow>
-             semPP (P||Q) now f g (Delay d, P'||Q', now+d, (\<lambda>t. if t \<le> now+d \<and> t \<ge> now then f' t else f t),
-                   (\<lambda>t. if t \<le> now+d \<and> t \<ge> now then g' t else g t))"
-(*| parallel4: "semP (Skip||Skip) now f (Tau, Skip, now, f)"*)
-
+| parallel3 : "semP P now f (Delay d, P', now + d, f')
+              \<and> semP Q now g (Delay d, Q', now + d, g') \<Longrightarrow>
+             semPP (P||Q) now f g (Delay d, P'||Q', now + d, (\<lambda>t. if t \<le> now + d \<and> t \<ge> now then f' t else f t),
+                (\<lambda>t. if t \<le> now + d \<and> t \<ge> now then g' t else g t))"
 
 text \<open>Big-step semantics\<close>
-
-inductive semB :: "proc \<Rightarrow> now \<Rightarrow> history \<Rightarrow> now \<Rightarrow> history \<Rightarrow> bool" where
+text \<open>Continuous evolution domain: assume b is an open formula, otherwise the escaping point cannot be found.\<close>
+inductive semB :: "'a :: finite proc \<Rightarrow> now \<Rightarrow> 'a history \<Rightarrow> now \<Rightarrow> 'a history \<Rightarrow> bool" where
   skipB: "semB Skip now f now f"
-| assignBR: "semB ((RVar x) := e) now f 
-    now (\<lambda>t. if t = now then (\<lambda> y. if y = x then evalE e (f t) else f t y) else f t)"
-| continuousBF: "([\<not>]b) (f now) \<Longrightarrow> semB (<[s]:E&&Inv&b>) now f now f"
-| continuousBT: "d>0 \<Longrightarrow> 
-       let f' = (\<lambda>t. if t \<le> now+d \<and> t > now then
-                       (\<lambda> y. if y = s then (Solution (Flow [s] E) (f now) (t-now)) else f now y)
-                     else f t)
-       in (\<forall>m. m < now+d \<and> m \<ge> now \<longrightarrow> b (f' m)) \<and> ([\<not>]b) (f' (now+d)) \<Longrightarrow>
-    semB (<[s]:E&&Inv&b>) now f (now+d)
-      (\<lambda>t. if t \<le> now+d \<and> t > now then
-             (\<lambda> y. if y = s then (Solution (Flow [s] E) (f now) (t-now)) else f now y)
-           else f t)"
+| assignB: "semB (x := e) now f 
+    now (\<lambda>t. if t = now then (update_fst (f t) x (evalE e (f t))) else f t)"
+| DassignB: "semB (DAss x e) now f 
+    now (\<lambda>t. if t = now then (update_snd (f t) x (evalE e (f t))) else f t)"
+(*| continuousBF: "let sol = ODE_solution ode 0 (f now) in
+      ([\<not>]b) (execute_ODE ode (f now) (sol 0)) \<Longrightarrow> semB (<ode && Inv&b>) now f 
+    now (\<lambda>t. if t = now then (execute_ODE ode (f now) ((ODE_solution ode 0 (f now)) 0))  else f t)"
+*)
+| continuous: "d \<ge> 0 \<Longrightarrow> ODE_solution ode d (f now) sol \<Longrightarrow>
+    (\<forall> t. t \<ge> 0 \<and> t < d \<longrightarrow> b (execute_ODE ode (f now) (sol t))) \<Longrightarrow> \<not> b (execute_ODE ode (f now) (sol d)) \<Longrightarrow>
+    semB (<ode && Inv&b>) now f 
+      (now + d) (\<lambda>t. if t \<le> now + d \<and> t \<ge> now then
+              (execute_ODE ode (f now) (sol (t-now)))  else f t)"
 | sequenceB: "semB P now f now' f' \<and> semB Q now' f' now'' f'' \<Longrightarrow> semB (P; Q) now f now'' f''"
 | conditionBT: " b (f now) \<Longrightarrow> semB P now f now_d f_d \<Longrightarrow> semB (IF b P) now f now_d f_d"
 | conditionBF: "\<not>b (f now) \<Longrightarrow> semB (IF b P) now f now f"
-| conditionGBT: " b (f now) \<Longrightarrow> semB P now f now_d f_d \<Longrightarrow> semB (IFELSE b P Q) now f now_d f_d"
-| conditionGBF: "\<not>b (f now) \<Longrightarrow> semB Q now f now_d f_d \<Longrightarrow> semB (IFELSE b P Q) now f now_d f_d"
-| joinBL: "semB P now f now_d f_d \<Longrightarrow> semB (P[[Q) now f now_d f_d"
-| joinBR: "semB Q now f now_d f_d \<Longrightarrow> semB (P[[Q) now f now_d f_d"
-| repetitionB: "\<exists>N. semB (P * NUM N) now f now_dd f_dd \<Longrightarrow> semB (P*&&Inv) now f now_dd f_dd"
+| IChoiceBL: "semB P now f now' f' \<Longrightarrow> semB (P \<sqinter> Q) now f now' f'"
+| IChoiceBR: "semB Q now f now' f' \<Longrightarrow> semB (P \<sqinter> Q) now f now' f'"
+| EChoiceL: "d \<ge> 0 \<Longrightarrow> semB P (now + d) (extend_history f now d) now' f' \<Longrightarrow>
+             semB (ch [!] e \<rightarrow> P [] dh [?] x \<rightarrow> Q) now f now' f'"
+| EChoiceR: "d \<ge> 0 \<Longrightarrow> semB (x := (Real c); Q) (now + d) (extend_history f now d) now' f' \<Longrightarrow>
+             semB (ch [!] e \<rightarrow> P [] dh [?] x \<rightarrow> Q) now f now' f'"
 | repetitionN0B: "N = (0::nat) \<Longrightarrow> semB (P * NUM N) now f now f"
 | repetitionNkB: "N > (0::nat) \<Longrightarrow> semB P now f now_d f_d \<Longrightarrow> semB (P * NUM (N-1)) now_d f_d now_dd f_dd \<Longrightarrow>
-                  semB (P * NUM N) now f now_dd f_dd"
-| outputBC: "d\<ge>0 \<Longrightarrow> semB (Cm (ch!!e)) now f (now+d) (\<lambda>t. if t \<le> now+d \<and> t > now then f now else f t)"
-| inputBC: "d\<ge>0 \<Longrightarrow> semB (Cm (ch??(RVar x))) now f (now + d)
-            (\<lambda>t. if t < now+d \<and> t > now then f now
-                 else if t = now+d then \<lambda> y. if y=x  then c else f now y
+                  semB (P * NUM N) now f now_dd f_dd" 
+| repetitionB: "\<exists>N. semB (P * NUM N) now f now_dd f_dd \<Longrightarrow> semB (P*&&Inv) now f now_dd f_dd"
+| outputBC: "d\<ge>0 \<Longrightarrow> semB (Cm (ch[!]e)) now f (now+d) (extend_history f now d)"
+| inputBC: "d\<ge>0 \<Longrightarrow> semB (Cm (ch[?]x)) now f (now + d)
+            (\<lambda>t. if t < now + d \<and> t > now then f now
+                 else if t = now + d then update_fst (f now) x c
                  else f t)"
+(*Notice: no real meaning of c in the inputBC. It will not be used actually without a synchronized output.*)
+ 
  
 text \<open>There are four cases for semantics of parallel composition.\<close>
-inductive semBP :: "procP \<Rightarrow> now \<Rightarrow> history \<Rightarrow> now \<Rightarrow> history \<Rightarrow> now \<Rightarrow> history \<Rightarrow> now \<Rightarrow> history \<Rightarrow> bool" where
+inductive semBP :: "'a ::finite procP \<Rightarrow> now \<Rightarrow> 'a history \<Rightarrow> now \<Rightarrow> 'a history \<Rightarrow> now \<Rightarrow> 'a history \<Rightarrow> now \<Rightarrow> 'a history \<Rightarrow> bool" where
   parallelB1: "semB P nowp fp nowp' fp' \<Longrightarrow> semB Q nowq fq nowq' fq' \<Longrightarrow> chanset P = {} \<and> chanset Q = {} \<Longrightarrow>
                semBP (P||Q) nowp fp nowq fq nowp' fp' nowq' fq'"
 | parallelB2: "semBP (P||Q) nowp fp nowq fq nowp' fp' nowq' fq' \<Longrightarrow>
                semB U nowp' fp' nowu' fu' \<Longrightarrow> semB V nowq' fq' nowv' fv' \<Longrightarrow> chanset P \<noteq> {} \<and> chanset Q \<noteq> {} \<Longrightarrow>
                chanset U = {} \<and> chanset V = {} \<Longrightarrow>
                semBP ((P; U) || (Q; V)) nowp fp nowq fq  nowu' fu' nowv' fv'"
-| parallelB3:
- "semBP (P || Q) nowp fp nowq fq nowp' fp' nowq' fq' \<Longrightarrow>
-  semBP (P; Cm (ch??(RVar x)) || Q; Cm (ch!!e)) nowp fp nowq fq (max nowp' nowq')
-   (\<lambda>t. if nowp' < t \<and> t < max nowp' nowq' then fp' nowp'
-         else if t = max nowp' nowq' then \<lambda> y. if y = x then evalE e (fp' nowp') else fp' nowp' y
+| parallelB3: "semBP (P || Q) nowp fp nowq fq nowp' fp' nowq' fq' \<Longrightarrow>
+    semBP (P; Cm (ch[?]x) || Q; Cm (ch[!]e)) nowp fp nowq fq (max nowp' nowq')
+     (\<lambda>t. if nowp' < t \<and> t < max nowp' nowq' then fp' nowp'
+         else if t = max nowp' nowq' then (update_fst (fp' nowp') x (evalE e (fp' nowp'))) 
               else fp' t)
-   (max nowp' nowq') (\<lambda>t. if nowq' < t \<and> t \<le> max nowp' nowq' then fq' nowq' else fq' t)"
-| parallelB4:
- "semBP (P || Q) nowp fp nowq fq nowp' fp' nowq' fq' \<Longrightarrow>
-  semBP (P; Cm (ch!!e) || Q; Cm (ch??(RVar x))) nowp fp nowq fq (max nowp' nowq')
+     (max nowp' nowq') (\<lambda>t. if nowq' < t \<and> t \<le> max nowp' nowq' then fq' nowq' else fq' t)"
+| parallelB4: "semBP (P || Q) nowp fp nowq fq nowp' fp' nowq' fq' \<Longrightarrow>
+  semBP (P; Cm (ch[!]e) || Q; Cm (ch[?]x)) nowp fp nowq fq (max nowp' nowq')
    (\<lambda>t. if nowp' < t \<and> t \<le> max nowp' nowq' then fp' nowp' else fp' t) (max nowp' nowq')
    (\<lambda>t. if nowq' < t \<and> t < max nowp' nowq' then fq' nowq'
-         else if t = max nowp' nowq' then \<lambda> y. if y = x then evalE e (fq' nowq') else fq' nowq' y
+         else if t = max nowp' nowq' then update_fst (fq' nowq') x (evalE e (fq' nowq'))
               else fq' t)"
-
+ 
 inductive_cases [elim!]:
   "semB Skip now f now' f'"
-  "semB ((RVar x) := e) now f now' f'"
-  "semB ((SVar x) := e) now f now' f'"
-  "semB ((BVar x) := e) now f now' f'"
+  "semB (DAss x e) now f now' f'"
+  "semB (x := e) now f now' f'"
   "semB (P; Q) now f now' f'"
-  "semB (IF be P) now f  now' f'"
-  "semB (IFELSE be P Q) now f now' f'"
-  "semB (P[[Q) now f now' f'"
-  "semB (<[s]:E&&Inv&b>) now f now' f'"
+  "semB (IF b P) now f  now' f'"
+  "semB (P \<sqinter> Q) now f now' f'"
+  "semB (<ode && Inv&b>) now f now' f'"
   "semB (P*&&Inv) now f now' f'"
   "semB (P* NUM N) now f now' f'"
+
+inductive_cases [elim!]:
   "semBP (P||Q) nowp fp nowq fq nowp' fp' nowq' fq'"
-
-
-subsection \<open>Continuous evolution\<close>
-
-(*Differential invariant: Now the invariant is annotated in the equation directly.*)
-(*consts Invariant :: "proc \<Rightarrow> fform"*)
-
-text \<open>exeFlow defines the execution of a continuous process from a state satisfying a given property\<close>
-definition exeFlow :: "proc \<Rightarrow> fform \<Rightarrow> fform" where
-  "exeFlow P p s \<equiv> (\<exists>now f now' f'. semB P now f now' f' \<and> p (f now) \<and> (\<exists>t. t \<le> now' \<and> t \<ge> now \<and> f' t = s))"
-
+ 
+ 
 
 subsection \<open>Properties related to semantics\<close>
 
@@ -198,11 +263,16 @@ lemma sem1:
   "semB P now f now' f' \<Longrightarrow> now \<le> now'"
   by (induct rule: semB.induct, auto)
 
+lemma semDass:
+  "semB (DAss x e) now f now' f' \<Longrightarrow> now' = now \<and> f' = (\<lambda>t. if t = now then update_snd (f t) x (evalE e (f t)) else f t)"
+  using semB.DassignB[of x e now f] by auto 
+
 lemma semB1:
   "semBP (P||Q) nowp fp nowq fq nowp' fp' nowq' fq' \<Longrightarrow> nowp \<le> nowp' \<and> nowq \<le> nowq'"
 proof (induct rule: semBP.induct)
   case (parallelB1 P nowp fp nowp' fp' Q nowq fq nowq' fq')
-  then show ?case by (auto intro: sem1)
+  then show ?case  
+    using sem1 by blast
 next
   case (parallelB2 P Q nowp fp nowq fq nowp' fp' nowq' fq' U nowu' fu' V nowv' fv')
   then show ?case by (metis order_trans sem1)
@@ -211,26 +281,31 @@ qed (metis le_max_iff_disj)+
 lemma sem2:
   "semB P now f now' f' \<Longrightarrow> \<forall>t. t < now \<or> t > now' \<longrightarrow> f t = f' t"
 proof (induct rule: semB.induct)
-  case (sequenceB P now f now' f' Q now'' f'')
-  then show ?case
-    by (metis (full_types) le_less_trans not_le sem1)
+   case (sequenceB P now f now' f' Q now'' f'')
+  then show ?case by (metis (full_types) le_less_trans not_le sem1)
+next
+   case (EChoiceL d P now f now' f' ch e dh x Q)
+  then show ?case 
+    by (smt extend_history.simps sem1)
+next
+  case (EChoiceR d x c Q now f now' f' ch e P dh)
+  then show ?case by (smt extend_history.simps sem1)
 next
   case (repetitionNkB N P now f now_d f_d now_dd f_dd)
-  then show ?case
-    by (metis (full_types) le_less_trans less_eq_real_def sem1)
+  then show ?case  by (metis (full_types) le_less_trans less_eq_real_def sem1)
 qed auto
-
+ 
 lemma semB2:
   "semBP (P||Q) nowp fp nowq fq nowp' fp' nowq' fq' \<Longrightarrow>
     (\<forall>t. t < nowp \<or> t > nowp' \<longrightarrow> (fp t = fp' t)) \<and>
     (\<forall>t. t < nowq \<or> t > nowq' \<longrightarrow> (fq t = fq' t))"
 proof (induct rule: semBP.induct)
   case (parallelB1 P nowp fp nowp' fp' Q nowq fq nowq' fq')
-  then show ?case by (auto simp add: sem2)
+  then show ?case  
+    using sem2 by blast
 next
   case (parallelB2 P Q nowp fp nowq fq nowp' fp' nowq' fq' U nowu' fu' V nowv' fv')
   then show ?case  by (smt sem1 sem2 semB1)
-
 next
   case (parallelB3 P Q nowp fp nowq fq nowp' fp' nowq' fq' ch x e)
   then show ?case by (smt semB1)
@@ -245,4 +320,6 @@ lemma semB3:
    semB P nowp fp nowp' fp' \<and> semB Q nowq fq nowq' fq'"
   by (induct rule: semBP.cases; simp add: chanset_def)
 
+ 
+ 
 end
