lunarlander/Syntax_SL.thy
@@ -1,75 +1,128 @@
 section \<open>Abstract syntax for Logic\<close>
 
 theory Syntax_SL 
-  imports Main HOL.Real
+  imports 
+    Main HOL.Real
+    Ordinary_Differential_Equations.ODE_Analysis
 begin
 
 text \<open>Expressions of HCSP language. \<close>
-datatype exp = Real real ("Real _" [75] 75)
-             | RVar string   ("RVar _" [75] 75)
-             | Add exp exp   (infixl "[+]" 70)
-             | Sub exp exp   (infixl "[-]" 70)
-             | Mul exp exp   (infixl "[*]" 71)
-             | Div exp exp   (infixl "[div]" 71)
-             | Pow exp nat   (infixl "[**]" 72)
+datatype 'a exp = Real real ("Real _" [75] 75)
+             | RVar 'a   ("RVar _" [75] 75)
+             | DVar 'a ("DVar _" [75] 75)
+             | Add "'a exp" "'a exp"   (infixl "[+]" 70)
+             | Sub "'a exp" "'a exp"   (infixl "[-]" 70)
+             | Mul "'a exp" "'a exp"   (infixl "[*]" 71)
+             | Diff "'a exp"  ("Diff _" [73] 73) 
 
- 
+
+
 text \<open>States\<close>
-type_synonym state = "string  \<Rightarrow> real"
+type_synonym 'a eval = "real^('a :: finite)"
+type_synonym 'a state = "'a eval"
+text \<open>A pair of states for recording variables and differential variables\<close>
+type_synonym 'a pair_state = "'a state \<times> 'a state"
 
-text \<open>Evaluation of expressions\<close>
-primrec evalE :: "exp \<Rightarrow> state \<Rightarrow> real" where
+definition Vagree :: "('a :: finite) pair_state \<Rightarrow> 'a pair_state \<Rightarrow> 'a set \<Rightarrow> bool"
+  where "Vagree u v V == 
+     (\<forall> i.  i \<in> V \<longrightarrow> fst u  $ i = fst v $ i \<and> snd u  $ i = snd v $ i)"
+
+lemma Vagree_eq:"Vagree \<nu> \<omega> UNIV \<Longrightarrow> \<nu> = \<omega>"
+  unfolding Vagree_def 
+  by (simp add: vec_eq_iff prod.expand)
+ 
+text \<open>Differential-free expressions\<close>
+primrec DE_free :: "('a :: finite) exp \<Rightarrow> bool" 
+  where
+  "DE_free (Real y)  = True"
+| "DE_free (RVar (x))  = True"
+| "DE_free (DVar (x))  = False"
+| "DE_free (e1 [+] e2)  = (DE_free e1  \<and> DE_free e2)"
+| "DE_free (e1 [-] e2)  = (DE_free e1  \<and> DE_free e2)"
+| "DE_free (e1 [*] e2)  = (DE_free e1  \<and> DE_free e2)"
+| "DE_free (Diff e)  = False" 
+
+text \<open>Evaluation of differential-free expressions\<close>
+primrec evalE_df :: "('a :: finite) exp \<Rightarrow> 'a state \<Rightarrow> real" 
+  where
+  "evalE_df (Real y) f = y"
+| "evalE_df (RVar (x)) f = f $ x"
+| "evalE_df (DVar (x)) f = undefined"
+| "evalE_df (e1 [+] e2) f = (evalE_df e1 f + evalE_df e2 f)"
+| "evalE_df (e1 [-] e2) f = (evalE_df e1 f - evalE_df e2 f)"
+| "evalE_df (e1 [*] e2) f = (evalE_df e1 f * evalE_df e2 f)"
+| "evalE_df (Diff e) f = undefined"  
+
+primrec frechet :: "'a :: finite exp \<Rightarrow> 'a state => 'a state => real"
+  where
+  "frechet (Real y) v = (\<lambda> v'. 0)"
+| "frechet (RVar x) v = (\<lambda> v'. v' \<bullet> axis x 1)"
+| "frechet (DVar x) v = undefined"
+| "frechet (e1 [+] e2) v = (\<lambda> v' . frechet e1 v v' + frechet e2 v v')"
+| "frechet (e1 [-] e2) v = (\<lambda> v' . frechet e1 v v' - frechet e2 v v')"
+| "frechet (e1 [*] e2) v = (\<lambda> v' . (evalE_df e1 v * frechet e2 v v' + frechet e1 v v' * evalE_df e2 v))"
+| "frechet (Diff e) v = undefined"
+
+
+text \<open>Evaluation of all expressions\<close>
+primrec evalE :: "'a :: finite exp \<Rightarrow> 'a pair_state \<Rightarrow> real" where
   "evalE (Real y) f = y"
-| "evalE (RVar (x)) f = f x"
+| "evalE (RVar (x)) f = (fst f) $ x"
+| "evalE (DVar (x)) f = (snd f) $ x"
 | "evalE (e1 [+] e2) f = (evalE e1 f + evalE e2 f)"
 | "evalE (e1 [-] e2) f = (evalE e1 f - evalE e2 f)"
 | "evalE (e1 [*] e2) f = (evalE e1 f * evalE e2 f)"
-| "evalE (e1 [div] e2) f = (evalE e1 f / evalE e2 f)"
-| "evalE (e1 [**] n) f = (evalE e1 f  ^ n)"
+| "evalE (Diff e) f = (frechet e (fst f) (snd f))"
+
+lemma DE_free_evalE: 
+ "DE_free e \<Longrightarrow> evalE e f = evalE_df e (fst f)"
+  by (induct e, auto)
 
 subsection \<open>FOL operators\<close>
 
-type_synonym fform = "state \<Rightarrow> bool"
+type_synonym 'a fform = "'a pair_state \<Rightarrow> bool"
 
-definition fTrue :: fform where "fTrue \<equiv> \<lambda>s. True"
-definition fFalse :: fform where "fFalse \<equiv> \<lambda>s. False"
+definition fTrue :: "'a fform" where "fTrue \<equiv> \<lambda>s. True"
+definition fFalse :: "'a fform" where "fFalse \<equiv> \<lambda>s. False"
 
-definition fEqual :: "exp \<Rightarrow> exp \<Rightarrow> fform"  (infixl "[=]" 50) where
+definition fEqual :: "'a :: finite exp \<Rightarrow> 'a exp \<Rightarrow> 'a fform"  (infixl "[=]" 50) where
   "e [=] f \<equiv> \<lambda>s. evalE e s = evalE f s"
 
-definition fLess :: "exp \<Rightarrow> exp \<Rightarrow> fform"  ("(_/ [<] _)"  [51, 51] 50) where
+definition fLess :: "'a :: finite exp \<Rightarrow> 'a exp \<Rightarrow> 'a fform"  ("(_/ [<] _)"  [51, 51] 50) where
   "e [<] f \<equiv> \<lambda>s. (evalE e s < evalE f s)"
 
-definition fAnd :: "fform \<Rightarrow> fform \<Rightarrow> fform"  (infixr "[&]" 35) where
+definition fAnd :: "'a fform \<Rightarrow> 'a fform \<Rightarrow> 'a fform"  (infixr "[&]" 35) where
   "P [&] Q \<equiv> \<lambda>s. P s \<and> Q s"
 
-definition fOr :: "fform \<Rightarrow> fform \<Rightarrow> fform"  (infixr "[|]" 30) where
+definition fOr :: "'a fform \<Rightarrow> 'a fform \<Rightarrow> 'a fform"  (infixr "[|]" 30) where
   "P [|] Q \<equiv> \<lambda>s. P s \<or> Q s"
 
-definition fNot :: "fform \<Rightarrow> fform"  ("[\<not>]_" [40] 40) where
+definition fNot :: "'a fform \<Rightarrow> 'a fform"  ("[\<not>]_" [40] 40) where
   "[\<not>]P \<equiv> \<lambda>s. \<not> P s"
 
-definition fImp :: "fform \<Rightarrow> fform \<Rightarrow> fform"  (infixr "[\<longrightarrow>]" 25) where
+definition fImp :: "'a fform \<Rightarrow> 'a fform \<Rightarrow> 'a fform"  (infixr "[\<longrightarrow>]" 25) where
   "P [\<longrightarrow>] Q \<equiv> \<lambda>s. P s \<longrightarrow> Q s"
 
-definition fLessEqual :: "exp \<Rightarrow> exp \<Rightarrow> fform"  ("(_/ [\<le>] _)"  [51, 51] 50) where
+definition fLessEqual :: "'a :: finite exp \<Rightarrow> 'a exp \<Rightarrow> 'a fform"  ("(_/ [\<le>] _)"  [51, 51] 50) where
   "e [\<le>] f \<equiv> (e [=] f) [|] (e [<] f)"
 
-definition fGreaterEqual :: "exp \<Rightarrow> exp \<Rightarrow> fform"   ("(_/ [\<ge>] _)"  [51, 51] 50) where
+definition fGreaterEqual :: "'a :: finite exp \<Rightarrow> 'a exp \<Rightarrow> 'a fform"   ("(_/ [\<ge>] _)"  [51, 51] 50) where
   "e [\<ge>] f \<equiv> \<lambda>s. ((evalE e s \<ge> evalE f s))"
 
-definition fGreater :: "exp \<Rightarrow> exp \<Rightarrow> fform"   ("(_/ [>] _)"  [51, 51] 50) where
+definition fGreater :: "'a :: finite exp \<Rightarrow> 'a exp \<Rightarrow> 'a fform"   ("(_/ [>] _)"  [51, 51] 50) where
   "e [>] f == [\<not>](e [\<le>] f)"
 
 
-text \<open>Evaluate on state after assigning value of expression e to (a, b).\<close>
-definition fSubForm :: "fform \<Rightarrow> exp \<Rightarrow> string \<Rightarrow> fform" ("_\<lbrakk>_,_\<rbrakk>" [71,71] 70) where
-  "P \<lbrakk>e, a\<rbrakk> \<equiv> (\<lambda>s. P (\<lambda> x. if x = a then evalE e s else s x))"
-
+text \<open>Evaluate on state after assigning value of expression e to RVar a.\<close>
+definition fSubForm :: "'a :: finite fform \<Rightarrow> 'a exp \<Rightarrow> 'a \<Rightarrow> 'a fform" ("_\<lbrakk>_,_\<rbrakk>" [71,71] 70) where
+  "P \<lbrakk>e, a\<rbrakk> \<equiv> (\<lambda>s. P (\<chi> x. if x = a then evalE e s else (fst s) $ x, snd s))"
+text \<open>Evaluate on state after assigning value of expression e to DVar a.\<close>
+definition fSubFormD :: "'a :: finite fform \<Rightarrow> 'a exp \<Rightarrow> 'a \<Rightarrow> 'a fform" ("_\<lbrakk>_,_\<rbrakk>\<^sub>D" [71,71] 70) where
+  "P \<lbrakk>e, a\<rbrakk>\<^sub>D \<equiv> (\<lambda>s. P (fst s, \<chi> x. if x = a then evalE e s else (snd s) $ x))"
 
 text \<open>The @{term close} operation extends the formula with the boundary,
   used for continuous evolution.\<close>
-axiomatization close :: "fform \<Rightarrow> fform" where
+axiomatization close :: "'a :: finite fform \<Rightarrow> 'a fform" where
   Lessc[simp]: "close (e [<] f) = (e [\<le>] f)" and
   Greatc[simp]: "close (e [>] f) = (e [\<ge>] f)" and
   Equalc[simp]: "close (e [=] f) = (e [=] f)" and
@@ -79,39 +132,53 @@ axiomatization close :: "fform \<Rightarrow> fform" where
   Orc[simp]: "close (P [|] Q) = (close (P) [|] close (Q))" and
   notLessc[simp]: "close ([\<not>] e [<] f) = (e [\<ge>] f)"
 
+
 declare fTrue_def [simp]
 declare fFalse_def [simp]
      
 text \<open>Types for defining HCSP\<close>
 type_synonym cname = string
 type_synonym time = real
+type_synonym var = string
 
 text \<open>Communication processes of HCSP\<close>
-datatype comm =
-  Send cname exp         ("_!!_" [110,108] 100)
-  | Receive cname exp      ("_??_" [110,108] 100)
+datatype 'a comm =
+  Send cname "'a exp"         ("_[!]_" [110,108] 100)
+  | Receive cname 'a      ("_[?]_" [110,108] 100)
 
+datatype 'a ODE =
+  ODEOne 'a "'a exp"  ("odeone _ _" [110,108] 100)
+  | ODEPar "'a ODE" "'a ODE"  ("odes _, _" [100,100] 90)
 
-
+fun ODE_vars :: "'a ODE \<Rightarrow> 'a set"
+  where
+  "ODE_vars (odeone x e) = { x }"
+| "ODE_vars (odes ode1, ode2) = ODE_vars ode1 \<union> ODE_vars ode2"
+ 
+fun wf_ODE :: "'a ODE \<Rightarrow> bool" 
+  where
+  "wf_ODE (odeone x e) = True"
+| "wf_ODE (odes ode1, ode2) = (ODE_vars ode1 \<inter> ODE_vars ode2 = {})"
+  
 text \<open>HCSP processes\<close>
-datatype proc =
-  Cm comm
+datatype 'a proc =
+  Cm "'a comm"
 | Skip
-| Ass exp exp             ("_ := _" [99,95] 94)
-| Seq proc proc           ("_; _" [91,90] 90)
-| Cond fform proc         ("IF _ _" [95,94] 93)
-| CondG fform proc proc   ("IFELSE _ _ _" [95,94,94] 93)
-| Pref comm proc          ("_\<rightarrow>_" [95,94] 93)
-| join proc proc          (infixr "[[" 90)
-| meet proc proc          ("_<<_" [90,90] 90)
+| Ass 'a "'a exp"             ("_ := _" [99,95] 94)
+| DAss 'a "'a exp"      
+| Seq "'a proc" "'a proc"           ("_; _" [91,90] 90)
+| Cond "'a fform" "'a proc"         ("IF _ _" [95,94] 93)
+(*| Pref comm proc          ("_\<rightarrow>_" [95,94] 93)*)
+| IChoice "'a proc" "'a proc"          (infixr "\<sqinter>" 90)
+| EChoice "'a comm" "'a proc" "'a comm" "'a proc"          ("_ \<rightarrow> _ [] _ \<rightarrow> _" [92,91,92,91] 90)
 \<comment> \<open>Repetition is annotated with invariant\<close>
-| Rep proc fform          ("_*&&_" [91] 90)
-| RepN proc nat           ("_* NUM _" [91, 90] 90)
+| Rep "'a proc" "'a fform"          ("_*&&_" [91] 90)
+| RepN "'a proc" nat           ("_* NUM _" [91, 90] 90)
 \<comment> \<open>Continuous evolution is annotated with invariant.\<close>
-| Cont "string list" "exp list" fform fform  ("<_:_&&_&_>" [95,95,96] 94)
-| Interp proc proc        ("_[[>_" [95,94] 94)
+| Cont "'a ODE" "'a fform" "'a fform"  ("<_&&_&_>" [95,95,96] 94)
+| Interr "'a proc" "'a comm" "'a proc"       ("_[]_\<rightarrow>_" [95,94,94] 94)
 
 text \<open>We assume parallel composition only occurs in the topmost level.\<close>
-datatype procP = Par proc proc  (infixr "||" 89)
+datatype 'a procP = Par "'a proc"  "'a proc"  (infixr "||" 89)
 
 end
